WIP

quotation/theories/ToTemplate/Coq/MSets.v
@@ -1,4 +1,3 @@
-Local Set Warnings Append "-masking-absolute-name".
 From Coq Require Import MSetInterface MSetList MSetAVL MSetFacts MSetProperties MSetDecide.
 From MetaCoq.Quotation.ToTemplate Require Export Init.
 From MetaCoq.Quotation.ToTemplate Require Export (hints) Coq.Numbers Coq.Init Coq.Lists Coq.Structures.
@@ -54,6 +53,26 @@ Module Type QuotationOfWSetsOn (E : DecidableType) (Import W : WSetsOn E).
   #[export] Declare Instance qchoose_spec2 : quotation_of choose_spec2.
 End QuotationOfWSetsOn.
 
+Module Type QuotationOfWSets (W : WSets) := QuotationOfWSetsOn W.E W.
+
+Module Type QuotationOfSetsOn (E : OrderedType) (Import M : SetsOn E).
+  Include QuotationOfWSetsOn E M.
+  #[export] Declare Instance qcompare : quotation_of M.compare.
+  #[export] Declare Instance qmin_elt : quotation_of M.min_elt.
+  #[export] Declare Instance qmax_elt : quotation_of M.max_elt.
+  #[export] Declare Instance qcompare_spec : quotation_of M.compare_spec.
+  #[export] Declare Instance qelements_spec2 : quotation_of M.elements_spec2.
+  #[export] Declare Instance qmin_elt_spec1 : quotation_of M.min_elt_spec1.
+  #[export] Declare Instance qmin_elt_spec2 : quotation_of M.min_elt_spec2.
+  #[export] Declare Instance qmin_elt_spec3 : quotation_of M.min_elt_spec3.
+  #[export] Declare Instance qmax_elt_spec1 : quotation_of M.max_elt_spec1.
+  #[export] Declare Instance qmax_elt_spec2 : quotation_of M.max_elt_spec2.
+  #[export] Declare Instance qmax_elt_spec3 : quotation_of M.max_elt_spec3.
+  #[export] Declare Instance qchoose_spec3 : quotation_of M.choose_spec3.
+End QuotationOfSetsOn.
+
+Module Type QuotationOfSets (M : Sets) := QuotationOfSetsOn M.E M.
+
 Module Type WFactsOnSig (E : DecidableType) (M : WSetsOn E) := Nop <+ WFactsOn E M.
 Module Type WFactsSig (M : WSets) := Nop <+ WFacts M.
 Module Type FactsSig (M : WSets) := Nop <+ Facts M.
@@ -65,323 +84,285 @@ Module Type WPropertiesSig (M : WSets) := Nop <+ WProperties M.
 Module Type PropertiesSig (M : WSets) := Nop <+ Properties M.
 Module Type OrdPropertiesSig (M : Sets) := Nop <+ OrdProperties M.
 
-(* the definitions *)
-Module ExtraQuotationOfWSetsOn (E : DecidableType) (Import W : WSetsOn E) (qE : QuotationOfDecidableType E) (Import qW : QuotationOfWSetsOn E W).
-  Import (hints) qE.
+Module Type QuotationOfWFactsOn (E : DecidableType) (M : WSetsOn E) (F : WFactsOnSig E M).
+  #[export] Declare Instance qeqb : quotation_of F.eqb.
+  #[export] Declare Instance qIn_1 : quotation_of F.In_1.
+  #[export] Declare Instance qmem_1 : quotation_of F.mem_1.
+  #[export] Declare Instance qmem_2 : quotation_of F.mem_2.
+  #[export] Declare Instance qequal_1 : quotation_of F.equal_1.
+  #[export] Declare Instance qequal_2 : quotation_of F.equal_2.
+  #[export] Declare Instance qsubset_1 : quotation_of F.subset_1.
+  #[export] Declare Instance qsubset_2 : quotation_of F.subset_2.
+  #[export] Declare Instance qis_empty_1 : quotation_of F.is_empty_1.
+  #[export] Declare Instance qis_empty_2 : quotation_of F.is_empty_2.
+  #[export] Declare Instance qadd_1 : quotation_of F.add_1.
+  #[export] Declare Instance qadd_2 : quotation_of F.add_2.
+  #[export] Declare Instance qadd_3 : quotation_of F.add_3.
+  #[export] Declare Instance qremove_1 : quotation_of F.remove_1.
+  #[export] Declare Instance qremove_2 : quotation_of F.remove_2.
+  #[export] Declare Instance qremove_3 : quotation_of F.remove_3.
+  #[export] Declare Instance qsingleton_1 : quotation_of F.singleton_1.
+  #[export] Declare Instance qsingleton_2 : quotation_of F.singleton_2.
+  #[export] Declare Instance qunion_1 : quotation_of F.union_1.
+  #[export] Declare Instance qunion_2 : quotation_of F.union_2.
+  #[export] Declare Instance qunion_3 : quotation_of F.union_3.
+  #[export] Declare Instance qinter_1 : quotation_of F.inter_1.
+  #[export] Declare Instance qinter_2 : quotation_of F.inter_2.
+  #[export] Declare Instance qinter_3 : quotation_of F.inter_3.
+  #[export] Declare Instance qdiff_1 : quotation_of F.diff_1.
+  #[export] Declare Instance qdiff_2 : quotation_of F.diff_2.
+  #[export] Declare Instance qdiff_3 : quotation_of F.diff_3.
+  #[export] Declare Instance qfilter_1 : quotation_of F.filter_1.
+  #[export] Declare Instance qfilter_2 : quotation_of F.filter_2.
+  #[export] Declare Instance qfilter_3 : quotation_of F.filter_3.
+  #[export] Declare Instance qfor_all_1 : quotation_of F.for_all_1.
+  #[export] Declare Instance qfor_all_2 : quotation_of F.for_all_2.
+  #[export] Declare Instance qexists_1 : quotation_of F.exists_1.
+  #[export] Declare Instance qexists_2 : quotation_of F.exists_2.
+  #[export] Declare Instance qelements_1 : quotation_of F.elements_1.
+  #[export] Declare Instance qelements_2 : quotation_of F.elements_2.
+  #[export] Declare Instance qIn_eq_iff : quotation_of F.In_eq_iff.
+  #[export] Declare Instance qmem_iff : quotation_of F.mem_iff.
+  #[export] Declare Instance qnot_mem_iff : quotation_of F.not_mem_iff.
+  #[export] Declare Instance qequal_iff : quotation_of F.equal_iff.
+  #[export] Declare Instance qsubset_iff : quotation_of F.subset_iff.
+  #[export] Declare Instance qempty_iff : quotation_of F.empty_iff.
+  #[export] Declare Instance qis_empty_iff : quotation_of F.is_empty_iff.
+  #[export] Declare Instance qsingleton_iff : quotation_of F.singleton_iff.
+  #[export] Declare Instance qadd_iff : quotation_of F.add_iff.
+  #[export] Declare Instance qadd_neq_iff : quotation_of F.add_neq_iff.
+  #[export] Declare Instance qremove_iff : quotation_of F.remove_iff.
+  #[export] Declare Instance qremove_neq_iff : quotation_of F.remove_neq_iff.
+  #[export] Declare Instance qfor_all_iff : quotation_of F.for_all_iff.
+  #[export] Declare Instance qexists_iff : quotation_of F.exists_iff.
+  #[export] Declare Instance qelements_iff : quotation_of F.elements_iff.
+  #[export] Declare Instance qmem_b : quotation_of F.mem_b.
+  #[export] Declare Instance qempty_b : quotation_of F.empty_b.
+  #[export] Declare Instance qadd_b : quotation_of F.add_b.
+  #[export] Declare Instance qadd_neq_b : quotation_of F.add_neq_b.
+  #[export] Declare Instance qremove_b : quotation_of F.remove_b.
+  #[export] Declare Instance qremove_neq_b : quotation_of F.remove_neq_b.
+  #[export] Declare Instance qsingleton_b : quotation_of F.singleton_b.
+  #[export] Declare Instance qunion_b : quotation_of F.union_b.
+  #[export] Declare Instance qinter_b : quotation_of F.inter_b.
+  #[export] Declare Instance qdiff_b : quotation_of F.diff_b.
+  #[export] Declare Instance qelements_b : quotation_of F.elements_b.
+  #[export] Declare Instance qfilter_b : quotation_of F.filter_b.
+  #[export] Declare Instance qfor_all_b : quotation_of F.for_all_b.
+  #[export] Declare Instance qexists_b : quotation_of F.exists_b.
+  #[export] Declare Instance qIn_m : quotation_of F.In_m.
+  #[export] Declare Instance qEmpty_m : quotation_of F.Empty_m.
+  #[export] Declare Instance qis_empty_m : quotation_of F.is_empty_m.
+  #[export] Declare Instance qmem_m : quotation_of F.mem_m.
+  #[export] Declare Instance qsingleton_m : quotation_of F.singleton_m.
+  #[export] Declare Instance qadd_m : quotation_of F.add_m.
+  #[export] Declare Instance qremove_m : quotation_of F.remove_m.
+  #[export] Declare Instance qunion_m : quotation_of F.union_m.
+  #[export] Declare Instance qinter_m : quotation_of F.inter_m.
+  #[export] Declare Instance qdiff_m : quotation_of F.diff_m.
+  #[export] Declare Instance qSubset_m : quotation_of F.Subset_m.
+  #[export] Declare Instance qsubset_m : quotation_of F.subset_m.
+  #[export] Declare Instance qequal_m : quotation_of F.equal_m.
+  #[export] Declare Instance qSubsetSetoid : quotation_of F.SubsetSetoid.
+  #[export] Declare Instance qSubset_refl : quotation_of F.Subset_refl.
+  #[export] Declare Instance qSubset_trans : quotation_of F.Subset_trans.
+  #[export] Declare Instance qIn_s_m : quotation_of F.In_s_m.
+  #[export] Declare Instance qEmpty_s_m : quotation_of F.Empty_s_m.
+  #[export] Declare Instance qadd_s_m : quotation_of F.add_s_m.
+  #[export] Declare Instance qremove_s_m : quotation_of F.remove_s_m.
+  #[export] Declare Instance qunion_s_m : quotation_of F.union_s_m.
+  #[export] Declare Instance qinter_s_m : quotation_of F.inter_s_m.
+  #[export] Declare Instance qdiff_s_m : quotation_of F.diff_s_m.
+  #[export] Declare Instance qfilter_equal : quotation_of (@F.filter_equal).
+  #[export] Declare Instance qfilter_subset : quotation_of (@F.filter_subset).
+  #[export] Declare Instance qfilter_ext : quotation_of F.filter_ext.
+End QuotationOfWFactsOn.
 
-  #[export] Instance qelt : quotation_of W.elt := ltac:(cbv [W.elt]; exact _).
-  #[export] Instance qEqual : quotation_of W.Equal := ltac:(cbv [W.Equal]; exact _).
-  #[export] Instance qSubset : quotation_of W.Subset := ltac:(cbv [W.Subset]; exact _).
-  #[export] Instance qEmpty : quotation_of W.Empty := ltac:(cbv [W.Empty]; exact _).
-  #[export] Instance qFor_all : quotation_of W.For_all := ltac:(cbv [W.For_all]; exact _).
-  #[export] Instance qExists : quotation_of W.Exists := ltac:(cbv [W.Exists]; exact _).
-  #[export] Instance qeq : quotation_of W.eq := ltac:(cbv [W.eq]; exact _).
+Module Type QuotationOfWFacts (M : WSets) (F : WFactsSig M) := QuotationOfWFactsOn M.E M F.
 
-  Module QuotationOfWFactsOn (WFacts : WFactsOnSig E W).
-    #[export] Instance qeqb : quotation_of WFacts.eqb := ltac:(unfold_quotation_of (); exact _).
-     #[export] Instance qIn_1 : quotation_of WFacts.In_1 := ltac:(unfold_quotation_of (); exact _).
-     #[export] Instance qmem_1 : quotation_of WFacts.mem_1 := ltac:(unfold_quotation_of (); exact _).
-     #[export] Instance qmem_2 : quotation_of WFacts.mem_2 := ltac:(unfold_quotation_of (); exact _).
-     #[export] Instance qequal_1 : quotation_of WFacts.equal_1 := ltac:(unfold_quotation_of (); exact _).
-     #[export] Instance qequal_2 : quotation_of WFacts.equal_2 := ltac:(unfold_quotation_of (); exact _).
-     #[export] Instance qsubset_1 : quotation_of WFacts.subset_1 := ltac:(unfold_quotation_of (); exact _).
-     #[export] Instance qsubset_2 : quotation_of WFacts.subset_2 := ltac:(unfold_quotation_of (); exact _).
-     #[export] Instance qis_empty_1 : quotation_of WFacts.is_empty_1 := ltac:(unfold_quotation_of (); exact _).
-     #[export] Instance qis_empty_2 : quotation_of WFacts.is_empty_2 := ltac:(unfold_quotation_of (); exact _).
-     #[export] Instance qadd_1 : quotation_of WFacts.add_1 := ltac:(unfold_quotation_of (); exact _).
-     #[export] Instance qadd_2 : quotation_of WFacts.add_2 := ltac:(unfold_quotation_of (); exact _).
-     #[export] Instance qadd_3 : quotation_of WFacts.add_3 := ltac:(unfold_quotation_of (); exact _).
-     #[export] Instance qremove_1 : quotation_of WFacts.remove_1 := ltac:(unfold_quotation_of (); exact _).
-     #[export] Instance qremove_2 : quotation_of WFacts.remove_2 := ltac:(unfold_quotation_of (); exact _).
-     #[export] Instance qremove_3 : quotation_of WFacts.remove_3 := ltac:(unfold_quotation_of (); exact _).
-     #[export] Instance qsingleton_1 : quotation_of WFacts.singleton_1 := ltac:(unfold_quotation_of (); exact _).
-     #[export] Instance qsingleton_2 : quotation_of WFacts.singleton_2 := ltac:(unfold_quotation_of (); exact _).
-     #[export] Instance qunion_1 : quotation_of WFacts.union_1 := ltac:(unfold_quotation_of (); exact _).
-     #[export] Instance qunion_2 : quotation_of WFacts.union_2 := ltac:(unfold_quotation_of (); exact _).
-     #[export] Instance qunion_3 : quotation_of WFacts.union_3 := ltac:(unfold_quotation_of (); exact _).
-     #[export] Instance qinter_1 : quotation_of WFacts.inter_1 := ltac:(unfold_quotation_of (); exact _).
-     #[export] Instance qinter_2 : quotation_of WFacts.inter_2 := ltac:(unfold_quotation_of (); exact _).
-     #[export] Instance qinter_3 : quotation_of WFacts.inter_3 := ltac:(unfold_quotation_of (); exact _).
-     #[export] Instance qdiff_1 : quotation_of WFacts.diff_1 := ltac:(unfold_quotation_of (); exact _).
-     #[export] Instance qdiff_2 : quotation_of WFacts.diff_2 := ltac:(unfold_quotation_of (); exact _).
-     #[export] Instance qdiff_3 : quotation_of WFacts.diff_3 := ltac:(unfold_quotation_of (); exact _).
-     #[export] Instance qfilter_1 : quotation_of WFacts.filter_1 := ltac:(unfold_quotation_of (); exact _).
-     #[export] Instance qfilter_2 : quotation_of WFacts.filter_2 := ltac:(unfold_quotation_of (); exact _).
-     #[export] Instance qfilter_3 : quotation_of WFacts.filter_3 := ltac:(unfold_quotation_of (); exact _).
-     #[export] Instance qfor_all_1 : quotation_of WFacts.for_all_1 := ltac:(unfold_quotation_of (); exact _).
-     #[export] Instance qfor_all_2 : quotation_of WFacts.for_all_2 := ltac:(unfold_quotation_of (); exact _).
-     #[export] Instance qexists_1 : quotation_of WFacts.exists_1 := ltac:(unfold_quotation_of (); exact _).
-     #[export] Instance qexists_2 : quotation_of WFacts.exists_2 := ltac:(unfold_quotation_of (); exact _).
-     #[export] Instance qelements_1 : quotation_of WFacts.elements_1 := ltac:(unfold_quotation_of (); exact _).
-     #[export] Instance qelements_2 : quotation_of WFacts.elements_2 := ltac:(unfold_quotation_of (); exact _).
-     #[export] Instance qIn_eq_iff : quotation_of WFacts.In_eq_iff := ltac:(unfold_quotation_of (); exact _).
-     #[export] Instance qmem_iff : quotation_of WFacts.mem_iff := ltac:(unfold_quotation_of (); exact _).
-     #[export] Instance qnot_mem_iff : quotation_of WFacts.not_mem_iff := ltac:(unfold_quotation_of (); exact _).
-     #[export] Instance qequal_iff : quotation_of WFacts.equal_iff := ltac:(unfold_quotation_of (); exact _).
-     #[export] Instance qsubset_iff : quotation_of WFacts.subset_iff := ltac:(unfold_quotation_of (); exact _).
-     #[export] Instance qempty_iff : quotation_of WFacts.empty_iff := ltac:(unfold_quotation_of (); exact _).
-     #[export] Instance qis_empty_iff : quotation_of WFacts.is_empty_iff := ltac:(unfold_quotation_of (); exact _).
-     #[export] Instance qsingleton_iff : quotation_of WFacts.singleton_iff := ltac:(unfold_quotation_of (); exact _).
-     #[export] Instance qadd_iff : quotation_of WFacts.add_iff := ltac:(unfold_quotation_of (); exact _).
-     #[export] Instance qadd_neq_iff : quotation_of WFacts.add_neq_iff := ltac:(unfold_quotation_of (); exact _).
-     #[export] Instance qremove_iff : quotation_of WFacts.remove_iff := ltac:(unfold_quotation_of (); exact _).
-     #[export] Instance qremove_neq_iff : quotation_of WFacts.remove_neq_iff := ltac:(unfold_quotation_of (); exact _).
-     #[export] Instance qfor_all_iff : quotation_of WFacts.for_all_iff := ltac:(unfold_quotation_of (); exact _).
-     #[export] Instance qexists_iff : quotation_of WFacts.exists_iff := ltac:(unfold_quotation_of (); exact _).
-     #[export] Instance qelements_iff : quotation_of WFacts.elements_iff := ltac:(unfold_quotation_of (); exact _).
-     #[export] Instance qmem_b : quotation_of WFacts.mem_b := ltac:(unfold_quotation_of (); exact _).
-     #[export] Instance qempty_b : quotation_of WFacts.empty_b := ltac:(unfold_quotation_of (); exact _).
-     (* too slow *)
-     (*
-     #[export] Instance qadd_b : quotation_of WFacts.add_b := ltac:(unfold_quotation_of (); exact _).
-     #[export] Instance qadd_neq_b : quotation_of WFacts.add_neq_b := ltac:(unfold_quotation_of (); exact _).
-     #[export] Instance qremove_b : quotation_of WFacts.remove_b := ltac:(unfold_quotation_of (); exact _).
-     #[export] Instance qremove_neq_b : quotation_of WFacts.remove_neq_b := ltac:(unfold_quotation_of (); exact _).
-     #[export] Instance qsingleton_b : quotation_of WFacts.singleton_b := ltac:(unfold_quotation_of (); exact _).
-     #[export] Instance qunion_b : quotation_of WFacts.union_b := ltac:(unfold_quotation_of (); exact _).
-     #[export] Instance qinter_b : quotation_of WFacts.inter_b := ltac:(unfold_quotation_of (); exact _).
-     #[export] Instance qdiff_b : quotation_of WFacts.diff_b := ltac:(unfold_quotation_of (); exact _).
-     #[export] Instance qelements_b : quotation_of WFacts.elements_b := ltac:(unfold_quotation_of (); exact _).
-     #[export] Instance qfilter_b : quotation_of WFacts.filter_b := ltac:(unfold_quotation_of (); exact _).
-     #[export] Instance qfor_all_b : quotation_of WFacts.for_all_b := ltac:(unfold_quotation_of (); exact _).
-     #[export] Instance qexists_b : quotation_of WFacts.exists_b := ltac:(unfold_quotation_of (); exact _).*)
-     #[export] Instance qIn_m : quotation_of WFacts.In_m := ltac:(unfold_quotation_of (); exact _).
-     #[export] Instance qEmpty_m : quotation_of WFacts.Empty_m := ltac:(unfold_quotation_of (); exact _).
-     (* too slow *)
-     (*
-     #[export] Instance qis_empty_m : quotation_of WFacts.is_empty_m := ltac:(unfold_quotation_of (); exact _).
-     #[export] Instance qmem_m : quotation_of WFacts.mem_m := ltac:(unfold_quotation_of (); exact _).
-     #[export] Instance qsingleton_m : quotation_of WFacts.singleton_m := ltac:(unfold_quotation_of (); exact _).
-     #[export] Instance qadd_m : quotation_of WFacts.add_m := ltac:(unfold_quotation_of (); exact _).
-     #[export] Instance qremove_m : quotation_of WFacts.remove_m := ltac:(unfold_quotation_of (); exact _).
-     #[export] Instance qunion_m : quotation_of WFacts.union_m := ltac:(unfold_quotation_of (); exact _).
-     #[export] Instance qinter_m : quotation_of WFacts.inter_m := ltac:(unfold_quotation_of (); exact _).
-     #[export] Instance qdiff_m : quotation_of WFacts.diff_m := ltac:(unfold_quotation_of (); exact _).
-     #[export] Instance qSubset_m : quotation_of WFacts.Subset_m := ltac:(unfold_quotation_of (); exact _).
-     #[export] Instance qsubset_m : quotation_of WFacts.subset_m := ltac:(unfold_quotation_of (); exact _).
-     #[export] Instance qequal_m : quotation_of WFacts.equal_m := ltac:(unfold_quotation_of (); exact _).
-     #[export] Instance qSubsetSetoid : quotation_of WFacts.SubsetSetoid := ltac:(unfold_quotation_of (); exact _).
-     #[export] Instance qSubset_refl : quotation_of WFacts.Subset_refl := ltac:(unfold_quotation_of (); exact _).
-     #[export] Instance qSubset_trans : quotation_of WFacts.Subset_trans := ltac:(unfold_quotation_of (); exact _).
-     #[export] Instance qIn_s_m : quotation_of WFacts.In_s_m := ltac:(unfold_quotation_of (); exact _).
-     #[export] Instance qEmpty_s_m : quotation_of WFacts.Empty_s_m := ltac:(unfold_quotation_of (); exact _).
-     #[export] Instance qadd_s_m : quotation_of WFacts.add_s_m := ltac:(unfold_quotation_of (); exact _).
-     #[export] Instance qremove_s_m : quotation_of WFacts.remove_s_m := ltac:(unfold_quotation_of (); exact _).
-     #[export] Instance qunion_s_m : quotation_of WFacts.union_s_m := ltac:(unfold_quotation_of (); exact _).
-     #[export] Instance qinter_s_m : quotation_of WFacts.inter_s_m := ltac:(unfold_quotation_of (); exact _).
-     #[export] Instance qdiff_s_m : quotation_of WFacts.diff_s_m := ltac:(unfold_quotation_of (); exact _).
-     #[export] Instance qfilter_equal : quotation_of WFacts.filter_equal := ltac:(unfold_quotation_of (); exact _).
-     #[export] Instance qfilter_subset : quotation_of WFacts.filter_subset := ltac:(unfold_quotation_of (); exact _).
-     #[export] Instance qfilter_ext : quotation_of WFacts.filter_ext := ltac:(unfold_quotation_of (); exact _).
-      *)
-  End QuotationOfWFactsOn.
+Module Type QuotationOfWDecideOn (E : DecidableType) (M : WSetsOn E) (F : WDecideOnSig E M).
+  Module qF := Nop <+ QuotationOfWFactsOn E M F.F.
+  Module qMSetDecideAuxiliary.
+    #[export] Declare Instance qMSet_elt_Prop : inductive_quotation_of F.MSetDecideAuxiliary.MSet_elt_Prop.
+    #[export] Declare Instance qMSet_Prop : inductive_quotation_of F.MSetDecideAuxiliary.MSet_Prop.
+    #[export] Declare Instance qeq_refl_iff : quotation_of F.MSetDecideAuxiliary.eq_refl_iff.
+    #[export] Declare Instance qdec_In : quotation_of F.MSetDecideAuxiliary.dec_In.
+    #[export] Declare Instance qdec_eq : quotation_of F.MSetDecideAuxiliary.dec_eq.
+  End qMSetDecideAuxiliary.
+  Export (hints) qF qMSetDecideAuxiliary.
+End QuotationOfWDecideOn.
 
-  Module QuotationOfWDecideOn (WDecide : WDecideOnSig E W).
-    Module qF := QuotationOfWFactsOn WDecide.F.
-    Export (hints) qF.
-    Module qMSetDecideAuxiliary.
-      (*#[export] Declare Instance qMSet_elt_Prop : inductive_quotation_of WDecide.MSetDecideAuxiliary.MSet_elt_Prop.
-      #[export] Declare Instance qMSet_Prop : inductive_quotation_of WDecide.MSetDecideAuxiliary.MSet_Prop.*)
-      #[export] Instance qeq_refl_iff : quotation_of WDecide.MSetDecideAuxiliary.eq_refl_iff := ltac:(unfold_quotation_of (); exact _).
-      #[export] Instance qdec_In : quotation_of WDecide.MSetDecideAuxiliary.dec_In := ltac:(unfold_quotation_of (); exact _).
-      #[export] Instance qdec_eq : quotation_of WDecide.MSetDecideAuxiliary.dec_eq := ltac:(unfold_quotation_of (); exact _).
-    End qMSetDecideAuxiliary.
-    Export (hints) qMSetDecideAuxiliary.
-  End QuotationOfWDecideOn.
+Module Type QuotationOfWDecide (M : WSets) (F : WDecideSig M) := QuotationOfWDecideOn M.E M F.
 
-  Module QuotationOfWPropertiesOn (WProperties : WPropertiesOnSig E W).
-    Module qDec := QuotationOfWDecideOn WProperties.Dec.
-    Export (hints) qDec.
-    #[export] Instance qIn_dec : quotation_of WProperties.In_dec := ltac:(unfold_quotation_of (); exact _).
-     #[export] Instance qAdd : quotation_of WProperties.Add := ltac:(unfold_quotation_of (); exact _).
-     #[export] Instance qAdd_Equal : quotation_of WProperties.Add_Equal := ltac:(unfold_quotation_of (); exact _).
-     #[export] Instance qequal_refl : quotation_of WProperties.equal_refl := ltac:(unfold_quotation_of (); exact _).
-     #[export] Instance qequal_sym : quotation_of WProperties.equal_sym := ltac:(unfold_quotation_of (); exact _).
-     #[export] Instance qequal_trans : quotation_of WProperties.equal_trans := ltac:(unfold_quotation_of (); exact _).
-     #[export] Instance qsubset_refl : quotation_of WProperties.subset_refl := ltac:(unfold_quotation_of (); exact _).
-     #[export] Instance qsubset_trans : quotation_of WProperties.subset_trans := ltac:(unfold_quotation_of (); exact _).
-     #[export] Instance qsubset_antisym : quotation_of WProperties.subset_antisym := ltac:(unfold_quotation_of (); exact _).
-     #[export] Instance qsubset_equal : quotation_of WProperties.subset_equal := ltac:(unfold_quotation_of (); exact _).
-     #[export] Instance qsubset_empty : quotation_of WProperties.subset_empty := ltac:(unfold_quotation_of (); exact _).
-     #[export] Instance qsubset_remove_3 : quotation_of WProperties.subset_remove_3 := ltac:(unfold_quotation_of (); exact _).
-     #[export] Instance qsubset_diff : quotation_of WProperties.subset_diff := ltac:(unfold_quotation_of (); exact _).
-     (*
-     #[export] Instance qsubset_add_3 : quotation_of WProperties.subset_add_3 := ltac:(unfold_quotation_of (); exact _).
-     #[export] Instance qsubset_add_2 : quotation_of WProperties.subset_add_2 := ltac:(unfold_quotation_of (); exact _).
-     #[export] Instance qin_subset : quotation_of WProperties.in_subset := ltac:(unfold_quotation_of (); exact _).
-     #[export] Instance qdouble_inclusion : quotation_of WProperties.double_inclusion := ltac:(unfold_quotation_of (); exact _).*)
-     #[export] Instance qempty_is_empty_1 : quotation_of WProperties.empty_is_empty_1 := ltac:(unfold_quotation_of (); exact _).
-     #[export] Instance qempty_is_empty_2 : quotation_of WProperties.empty_is_empty_2 := ltac:(unfold_quotation_of (); exact _).
-     (*
-     #[export] Instance qadd_equal : quotation_of WProperties.add_equal := ltac:(unfold_quotation_of (); exact _).
-     #[export] Instance qadd_add : quotation_of WProperties.add_add := ltac:(unfold_quotation_of (); exact _).
-     #[export] Instance qremove_equal : quotation_of WProperties.remove_equal := ltac:(unfold_quotation_of (); exact _).
-     #[export] Instance qEqual_remove : quotation_of WProperties.Equal_remove := ltac:(unfold_quotation_of (); exact _).
-     #[export] Instance qadd_remove : quotation_of WProperties.add_remove := ltac:(unfold_quotation_of (); exact _).
-     #[export] Instance qremove_add : quotation_of WProperties.remove_add := ltac:(unfold_quotation_of (); exact _).
-     #[export] Instance qsingleton_equal_add : quotation_of WProperties.singleton_equal_add := ltac:(unfold_quotation_of (); exact _).
-     #[export] Instance qremove_singleton_empty : quotation_of WProperties.remove_singleton_empty := ltac:(unfold_quotation_of (); exact _).
-     #[export] Instance qunion_sym : quotation_of WProperties.union_sym := ltac:(unfold_quotation_of (); exact _).
-     #[export] Instance qunion_subset_equal : quotation_of WProperties.union_subset_equal := ltac:(unfold_quotation_of (); exact _).
-     #[export] Instance qunion_equal_1 : quotation_of WProperties.union_equal_1 := ltac:(unfold_quotation_of (); exact _).
-     #[export] Instance qunion_equal_2 : quotation_of WProperties.union_equal_2 := ltac:(unfold_quotation_of (); exact _).
-     #[export] Instance qunion_assoc : quotation_of WProperties.union_assoc := ltac:(unfold_quotation_of (); exact _).
-     #[export] Instance qadd_union_singleton : quotation_of WProperties.add_union_singleton := ltac:(unfold_quotation_of (); exact _).
-     #[export] Instance qunion_add : quotation_of WProperties.union_add := ltac:(unfold_quotation_of (); exact _).
-     #[export] Instance qunion_remove_add_1 : quotation_of WProperties.union_remove_add_1 := ltac:(unfold_quotation_of (); exact _).
-     #[export] Instance qunion_remove_add_2 : quotation_of WProperties.union_remove_add_2 := ltac:(unfold_quotation_of (); exact _).
-     #[export] Instance qunion_subset_1 : quotation_of WProperties.union_subset_1 := ltac:(unfold_quotation_of (); exact _).
-     #[export] Instance qunion_subset_2 : quotation_of WProperties.union_subset_2 := ltac:(unfold_quotation_of (); exact _).
-     #[export] Instance qunion_subset_3 : quotation_of WProperties.union_subset_3 := ltac:(unfold_quotation_of (); exact _).
-     #[export] Instance qunion_subset_4 : quotation_of WProperties.union_subset_4 := ltac:(unfold_quotation_of (); exact _).
-     #[export] Instance qunion_subset_5 : quotation_of WProperties.union_subset_5 := ltac:(unfold_quotation_of (); exact _).
-     #[export] Instance qempty_union_1 : quotation_of WProperties.empty_union_1 := ltac:(unfold_quotation_of (); exact _).
-     #[export] Instance qempty_union_2 : quotation_of WProperties.empty_union_2 := ltac:(unfold_quotation_of (); exact _).
-     #[export] Instance qnot_in_union : quotation_of WProperties.not_in_union := ltac:(unfold_quotation_of (); exact _).
-     #[export] Instance qinter_sym : quotation_of WProperties.inter_sym := ltac:(unfold_quotation_of (); exact _).
-     #[export] Instance qinter_subset_equal : quotation_of WProperties.inter_subset_equal := ltac:(unfold_quotation_of (); exact _).
-     #[export] Instance qinter_equal_1 : quotation_of WProperties.inter_equal_1 := ltac:(unfold_quotation_of (); exact _).
-     #[export] Instance qinter_equal_2 : quotation_of WProperties.inter_equal_2 := ltac:(unfold_quotation_of (); exact _).
-     #[export] Instance qinter_assoc : quotation_of WProperties.inter_assoc := ltac:(unfold_quotation_of (); exact _).
-     #[export] Instance qunion_inter_1 : quotation_of WProperties.union_inter_1 := ltac:(unfold_quotation_of (); exact _).
-     #[export] Instance qunion_inter_2 : quotation_of WProperties.union_inter_2 := ltac:(unfold_quotation_of (); exact _).
-     #[export] Instance qinter_add_1 : quotation_of WProperties.inter_add_1 := ltac:(unfold_quotation_of (); exact _).
-     #[export] Instance qinter_add_2 : quotation_of WProperties.inter_add_2 := ltac:(unfold_quotation_of (); exact _).
-     #[export] Instance qempty_inter_1 : quotation_of WProperties.empty_inter_1 := ltac:(unfold_quotation_of (); exact _).
-     #[export] Instance qempty_inter_2 : quotation_of WProperties.empty_inter_2 := ltac:(unfold_quotation_of (); exact _).
-     #[export] Instance qinter_subset_1 : quotation_of WProperties.inter_subset_1 := ltac:(unfold_quotation_of (); exact _).
-     #[export] Instance qinter_subset_2 : quotation_of WProperties.inter_subset_2 := ltac:(unfold_quotation_of (); exact _).
-     #[export] Instance qinter_subset_3 : quotation_of WProperties.inter_subset_3 := ltac:(unfold_quotation_of (); exact _).
-     #[export] Instance qempty_diff_1 : quotation_of WProperties.empty_diff_1 := ltac:(unfold_quotation_of (); exact _).
-     #[export] Instance qempty_diff_2 : quotation_of WProperties.empty_diff_2 := ltac:(unfold_quotation_of (); exact _).
-     #[export] Instance qdiff_subset : quotation_of WProperties.diff_subset := ltac:(unfold_quotation_of (); exact _).
-     #[export] Instance qdiff_subset_equal : quotation_of WProperties.diff_subset_equal := ltac:(unfold_quotation_of (); exact _).
-     #[export] Instance qremove_diff_singleton : quotation_of WProperties.remove_diff_singleton := ltac:(unfold_quotation_of (); exact _).
-     #[export] Instance qdiff_inter_empty : quotation_of WProperties.diff_inter_empty := ltac:(unfold_quotation_of (); exact _).
-     #[export] Instance qdiff_inter_all : quotation_of WProperties.diff_inter_all := ltac:(unfold_quotation_of (); exact _).
-     #[export] Instance qAdd_add : quotation_of WProperties.Add_add := ltac:(unfold_quotation_of (); exact _).
-     #[export] Instance qAdd_remove : quotation_of WProperties.Add_remove := ltac:(unfold_quotation_of (); exact _).
-     #[export] Instance qunion_Add : quotation_of WProperties.union_Add := ltac:(unfold_quotation_of (); exact _).
-     #[export] Instance qinter_Add : quotation_of WProperties.inter_Add := ltac:(unfold_quotation_of (); exact _).
-     #[export] Instance qunion_Equal : quotation_of WProperties.union_Equal := ltac:(unfold_quotation_of (); exact _).
-     #[export] Instance qinter_Add_2 : quotation_of WProperties.inter_Add_2 := ltac:(unfold_quotation_of (); exact _).
-     #[export] Instance qelements_Empty : quotation_of WProperties.elements_Empty := ltac:(unfold_quotation_of (); exact _).
-     #[export] Instance qelements_empty : quotation_of WProperties.elements_empty := ltac:(unfold_quotation_of (); exact _).
-     #[export] Instance qof_list : quotation_of WProperties.of_list := ltac:(unfold_quotation_of (); exact _).
-     #[export] Instance qto_list : quotation_of WProperties.to_list := ltac:(unfold_quotation_of (); exact _).
-     #[export] Instance qof_list_1 : quotation_of WProperties.of_list_1 := ltac:(unfold_quotation_of (); exact _).
-     #[export] Instance qof_list_2 : quotation_of WProperties.of_list_2 := ltac:(unfold_quotation_of (); exact _).
-     #[export] Instance qof_list_3 : quotation_of WProperties.of_list_3 := ltac:(unfold_quotation_of (); exact _).
-     #[export] Instance qfold_spec_right : quotation_of WProperties.fold_spec_right := ltac:(unfold_quotation_of (); exact _).
-     #[export] Instance qfold_rec : quotation_of WProperties.fold_rec := ltac:(unfold_quotation_of (); exact _).
-     #[export] Instance qfold_rec_bis : quotation_of WProperties.fold_rec_bis := ltac:(unfold_quotation_of (); exact _).
-     #[export] Instance qfold_rec_nodep : quotation_of WProperties.fold_rec_nodep := ltac:(unfold_quotation_of (); exact _).
-     #[export] Instance qfold_rec_weak : quotation_of WProperties.fold_rec_weak := ltac:(unfold_quotation_of (); exact _).
-     #[export] Instance qfold_rel : quotation_of WProperties.fold_rel := ltac:(unfold_quotation_of (); exact _).
-     #[export] Instance qset_induction : quotation_of WProperties.set_induction := ltac:(unfold_quotation_of (); exact _).
-     #[export] Instance qset_induction_bis : quotation_of WProperties.set_induction_bis := ltac:(unfold_quotation_of (); exact _).
-     #[export] Instance qfold_identity : quotation_of WProperties.fold_identity := ltac:(unfold_quotation_of (); exact _).
-     #[export] Instance qfold_0 : quotation_of WProperties.fold_0 := ltac:(unfold_quotation_of (); exact _).
-     #[export] Instance qfold_1 : quotation_of WProperties.fold_1 := ltac:(unfold_quotation_of (); exact _).
-     #[export] Instance qfold_2 : quotation_of WProperties.fold_2 := ltac:(unfold_quotation_of (); exact _).
-     #[export] Instance qfold_1b : quotation_of WProperties.fold_1b := ltac:(unfold_quotation_of (); exact _).
-     #[export] Instance qfold_commutes : quotation_of WProperties.fold_commutes := ltac:(unfold_quotation_of (); exact _).
-     #[export] Instance qfold_init : quotation_of WProperties.fold_init := ltac:(unfold_quotation_of (); exact _).
-     #[export] Instance qfold_equal : quotation_of WProperties.fold_equal := ltac:(unfold_quotation_of (); exact _).
-     #[export] Instance qfold_empty : quotation_of WProperties.fold_empty := ltac:(unfold_quotation_of (); exact _).
-     #[export] Instance qfold_add : quotation_of WProperties.fold_add := ltac:(unfold_quotation_of (); exact _).
-     #[export] Instance qadd_fold : quotation_of WProperties.add_fold := ltac:(unfold_quotation_of (); exact _).
-     #[export] Instance qremove_fold_1 : quotation_of WProperties.remove_fold_1 := ltac:(unfold_quotation_of (); exact _).
-     #[export] Instance qremove_fold_2 : quotation_of WProperties.remove_fold_2 := ltac:(unfold_quotation_of (); exact _).
-     #[export] Instance qfold_union_inter : quotation_of WProperties.fold_union_inter := ltac:(unfold_quotation_of (); exact _).
-     #[export] Instance qfold_diff_inter : quotation_of WProperties.fold_diff_inter := ltac:(unfold_quotation_of (); exact _).
-     #[export] Instance qfold_union : quotation_of WProperties.fold_union := ltac:(unfold_quotation_of (); exact _).
-     #[export] Instance qfold_plus : quotation_of WProperties.fold_plus := ltac:(unfold_quotation_of (); exact _).
-     #[export] Instance qcardinal_fold : quotation_of WProperties.cardinal_fold := ltac:(unfold_quotation_of (); exact _).
-     #[export] Instance qcardinal_0 : quotation_of WProperties.cardinal_0 := ltac:(unfold_quotation_of (); exact _).
-     #[export] Instance qcardinal_1 : quotation_of WProperties.cardinal_1 := ltac:(unfold_quotation_of (); exact _).
-     #[export] Instance qcardinal_2 : quotation_of WProperties.cardinal_2 := ltac:(unfold_quotation_of (); exact _).
-     #[export] Instance qcardinal_Empty : quotation_of WProperties.cardinal_Empty := ltac:(unfold_quotation_of (); exact _).
-     #[export] Instance qcardinal_inv_1 : quotation_of WProperties.cardinal_inv_1 := ltac:(unfold_quotation_of (); exact _).
-     #[export] Instance qcardinal_inv_2 : quotation_of WProperties.cardinal_inv_2 := ltac:(unfold_quotation_of (); exact _).
-     #[export] Instance qcardinal_inv_2b : quotation_of WProperties.cardinal_inv_2b := ltac:(unfold_quotation_of (); exact _).
-     #[export] Instance qEqual_cardinal : quotation_of WProperties.Equal_cardinal := ltac:(unfold_quotation_of (); exact _).
-     #[export] Instance qcardinal_m : quotation_of WProperties.cardinal_m := ltac:(unfold_quotation_of (); exact _).
-     #[export] Instance qempty_cardinal : quotation_of WProperties.empty_cardinal := ltac:(unfold_quotation_of (); exact _).
-     #[export] Instance qsingleton_cardinal : quotation_of WProperties.singleton_cardinal := ltac:(unfold_quotation_of (); exact _).
-     #[export] Instance qdiff_inter_cardinal : quotation_of WProperties.diff_inter_cardinal := ltac:(unfold_quotation_of (); exact _).
-     #[export] Instance qunion_cardinal : quotation_of WProperties.union_cardinal := ltac:(unfold_quotation_of (); exact _).
-     #[export] Instance qsubset_cardinal : quotation_of WProperties.subset_cardinal := ltac:(unfold_quotation_of (); exact _).
-     #[export] Instance qsubset_cardinal_lt : quotation_of WProperties.subset_cardinal_lt := ltac:(unfold_quotation_of (); exact _).
-     #[export] Instance qunion_inter_cardinal : quotation_of WProperties.union_inter_cardinal := ltac:(unfold_quotation_of (); exact _).
-     #[export] Instance qunion_cardinal_inter : quotation_of WProperties.union_cardinal_inter := ltac:(unfold_quotation_of (); exact _).
-     #[export] Instance qunion_cardinal_le : quotation_of WProperties.union_cardinal_le := ltac:(unfold_quotation_of (); exact _).
-     #[export] Instance qadd_cardinal_1 : quotation_of WProperties.add_cardinal_1 := ltac:(unfold_quotation_of (); exact _).
-     #[export] Instance qadd_cardinal_2 : quotation_of WProperties.add_cardinal_2 := ltac:(unfold_quotation_of (); exact _).
-     #[export] Instance qremove_cardinal_1 : quotation_of WProperties.remove_cardinal_1 := ltac:(unfold_quotation_of (); exact _).
-     #[export] Instance qremove_cardinal_2 : quotation_of WProperties.remove_cardinal_2 := ltac:(unfold_quotation_of (); exact _).*)
-  End QuotationOfWPropertiesOn.
-End ExtraQuotationOfWSetsOn.
+Module Type QuotationOfWPropertiesOn (E : DecidableType) (M : WSetsOn E) (F : WPropertiesOnSig E M).
+  Module qDec := Nop <+ QuotationOfWDecideOn E M F.Dec.
+  Module qFM := Nop <+ QuotationOfWFactsOn E M F.FM.
+  Export (hints) qDec qFM.
+  #[export] Declare Instance qIn_dec : quotation_of F.In_dec.
+  #[export] Declare Instance qAdd : quotation_of F.Add.
+  #[export] Declare Instance qAdd_Equal : quotation_of F.Add_Equal.
+  #[export] Declare Instance qequal_refl : quotation_of F.equal_refl.
+  #[export] Declare Instance qequal_sym : quotation_of F.equal_sym.
+  #[export] Declare Instance qequal_trans : quotation_of F.equal_trans.
+  #[export] Declare Instance qsubset_refl : quotation_of F.subset_refl.
+  #[export] Declare Instance qsubset_trans : quotation_of F.subset_trans.
+  #[export] Declare Instance qsubset_antisym : quotation_of F.subset_antisym.
+  #[export] Declare Instance qsubset_equal : quotation_of F.subset_equal.
+  #[export] Declare Instance qsubset_empty : quotation_of F.subset_empty.
+  #[export] Declare Instance qsubset_remove_3 : quotation_of F.subset_remove_3.
+  #[export] Declare Instance qsubset_diff : quotation_of F.subset_diff.
+  #[export] Declare Instance qsubset_add_3 : quotation_of F.subset_add_3.
+  #[export] Declare Instance qsubset_add_2 : quotation_of F.subset_add_2.
+  #[export] Declare Instance qin_subset : quotation_of F.in_subset.
+  #[export] Declare Instance qdouble_inclusion : quotation_of F.double_inclusion.
+  #[export] Declare Instance qempty_is_empty_1 : quotation_of F.empty_is_empty_1.
+  #[export] Declare Instance qempty_is_empty_2 : quotation_of F.empty_is_empty_2.
+  #[export] Declare Instance qadd_equal : quotation_of F.add_equal.
+  #[export] Declare Instance qadd_add : quotation_of F.add_add.
+  #[export] Declare Instance qremove_equal : quotation_of F.remove_equal.
+  #[export] Declare Instance qEqual_remove : quotation_of F.Equal_remove.
+  #[export] Declare Instance qadd_remove : quotation_of F.add_remove.
+  #[export] Declare Instance qremove_add : quotation_of F.remove_add.
+  #[export] Declare Instance qsingleton_equal_add : quotation_of F.singleton_equal_add.
+  #[export] Declare Instance qremove_singleton_empty : quotation_of F.remove_singleton_empty.
+  #[export] Declare Instance qunion_sym : quotation_of F.union_sym.
+  #[export] Declare Instance qunion_subset_equal : quotation_of F.union_subset_equal.
+  #[export] Declare Instance qunion_equal_1 : quotation_of F.union_equal_1.
+  #[export] Declare Instance qunion_equal_2 : quotation_of F.union_equal_2.
+  #[export] Declare Instance qunion_assoc : quotation_of F.union_assoc.
+  #[export] Declare Instance qadd_union_singleton : quotation_of F.add_union_singleton.
+  #[export] Declare Instance qunion_add : quotation_of F.union_add.
+  #[export] Declare Instance qunion_remove_add_1 : quotation_of F.union_remove_add_1.
+  #[export] Declare Instance qunion_remove_add_2 : quotation_of F.union_remove_add_2.
+  #[export] Declare Instance qunion_subset_1 : quotation_of F.union_subset_1.
+  #[export] Declare Instance qunion_subset_2 : quotation_of F.union_subset_2.
+  #[export] Declare Instance qunion_subset_3 : quotation_of F.union_subset_3.
+  #[export] Declare Instance qunion_subset_4 : quotation_of F.union_subset_4.
+  #[export] Declare Instance qunion_subset_5 : quotation_of F.union_subset_5.
+  #[export] Declare Instance qempty_union_1 : quotation_of F.empty_union_1.
+  #[export] Declare Instance qempty_union_2 : quotation_of F.empty_union_2.
+  #[export] Declare Instance qnot_in_union : quotation_of F.not_in_union.
+  #[export] Declare Instance qinter_sym : quotation_of F.inter_sym.
+  #[export] Declare Instance qinter_subset_equal : quotation_of F.inter_subset_equal.
+  #[export] Declare Instance qinter_equal_1 : quotation_of F.inter_equal_1.
+  #[export] Declare Instance qinter_equal_2 : quotation_of F.inter_equal_2.
+  #[export] Declare Instance qinter_assoc : quotation_of F.inter_assoc.
+  #[export] Declare Instance qunion_inter_1 : quotation_of F.union_inter_1.
+  #[export] Declare Instance qunion_inter_2 : quotation_of F.union_inter_2.
+  #[export] Declare Instance qinter_add_1 : quotation_of F.inter_add_1.
+  #[export] Declare Instance qinter_add_2 : quotation_of F.inter_add_2.
+  #[export] Declare Instance qempty_inter_1 : quotation_of F.empty_inter_1.
+  #[export] Declare Instance qempty_inter_2 : quotation_of F.empty_inter_2.
+  #[export] Declare Instance qinter_subset_1 : quotation_of F.inter_subset_1.
+  #[export] Declare Instance qinter_subset_2 : quotation_of F.inter_subset_2.
+  #[export] Declare Instance qinter_subset_3 : quotation_of F.inter_subset_3.
+  #[export] Declare Instance qempty_diff_1 : quotation_of F.empty_diff_1.
+  #[export] Declare Instance qempty_diff_2 : quotation_of F.empty_diff_2.
+  #[export] Declare Instance qdiff_subset : quotation_of F.diff_subset.
+  #[export] Declare Instance qdiff_subset_equal : quotation_of F.diff_subset_equal.
+  #[export] Declare Instance qremove_diff_singleton : quotation_of F.remove_diff_singleton.
+  #[export] Declare Instance qdiff_inter_empty : quotation_of F.diff_inter_empty.
+  #[export] Declare Instance qdiff_inter_all : quotation_of F.diff_inter_all.
+  #[export] Declare Instance qAdd_add : quotation_of F.Add_add.
+  #[export] Declare Instance qAdd_remove : quotation_of F.Add_remove.
+  #[export] Declare Instance qunion_Add : quotation_of F.union_Add.
+  #[export] Declare Instance qinter_Add : quotation_of F.inter_Add.
+  #[export] Declare Instance qunion_Equal : quotation_of F.union_Equal.
+  #[export] Declare Instance qinter_Add_2 : quotation_of F.inter_Add_2.
+  #[export] Declare Instance qelements_Empty : quotation_of F.elements_Empty.
+  #[export] Declare Instance qelements_empty : quotation_of F.elements_empty.
+  #[export] Declare Instance qof_list : quotation_of F.of_list.
+  #[export] Declare Instance qto_list : quotation_of F.to_list.
+  #[export] Declare Instance qof_list_1 : quotation_of F.of_list_1.
+  #[export] Declare Instance qof_list_2 : quotation_of F.of_list_2.
+  #[export] Declare Instance qof_list_3 : quotation_of F.of_list_3.
+  #[export] Declare Instance qfold_spec_right : quotation_of F.fold_spec_right.
+  #[export] Declare Instance qfold_rec : quotation_of F.fold_rec.
+  #[export] Declare Instance qfold_rec_bis : quotation_of F.fold_rec_bis.
+  #[export] Declare Instance qfold_rec_nodep : quotation_of F.fold_rec_nodep.
+  #[export] Declare Instance qfold_rec_weak : quotation_of F.fold_rec_weak.
+  #[export] Declare Instance qfold_rel : quotation_of F.fold_rel.
+  #[export] Declare Instance qset_induction : quotation_of F.set_induction.
+  #[export] Declare Instance qset_induction_bis : quotation_of F.set_induction_bis.
+  #[export] Declare Instance qfold_identity : quotation_of F.fold_identity.
+  #[export] Declare Instance qfold_0 : quotation_of F.fold_0.
+  #[export] Declare Instance qfold_1 : quotation_of F.fold_1.
+  #[export] Declare Instance qfold_2 : quotation_of F.fold_2.
+  #[export] Declare Instance qfold_1b : quotation_of F.fold_1b.
+  #[export] Declare Instance qfold_commutes : quotation_of F.fold_commutes.
+  #[export] Declare Instance qfold_init : quotation_of F.fold_init.
+  #[export] Declare Instance qfold_equal : quotation_of F.fold_equal.
+  #[export] Declare Instance qfold_empty : quotation_of F.fold_empty.
+  #[export] Declare Instance qfold_add : quotation_of F.fold_add.
+  #[export] Declare Instance qadd_fold : quotation_of F.add_fold.
+  #[export] Declare Instance qremove_fold_1 : quotation_of F.remove_fold_1.
+  #[export] Declare Instance qremove_fold_2 : quotation_of F.remove_fold_2.
+  #[export] Declare Instance qfold_union_inter : quotation_of F.fold_union_inter.
+  #[export] Declare Instance qfold_diff_inter : quotation_of F.fold_diff_inter.
+  #[export] Declare Instance qfold_union : quotation_of F.fold_union.
+  #[export] Declare Instance qfold_plus : quotation_of F.fold_plus.
+  #[export] Declare Instance qcardinal_fold : quotation_of F.cardinal_fold.
+  #[export] Declare Instance qcardinal_0 : quotation_of F.cardinal_0.
+  #[export] Declare Instance qcardinal_1 : quotation_of F.cardinal_1.
+  #[export] Declare Instance qcardinal_2 : quotation_of F.cardinal_2.
+  #[export] Declare Instance qcardinal_Empty : quotation_of F.cardinal_Empty.
+  #[export] Declare Instance qcardinal_inv_1 : quotation_of F.cardinal_inv_1.
+  #[export] Declare Instance qcardinal_inv_2 : quotation_of F.cardinal_inv_2.
+  #[export] Declare Instance qcardinal_inv_2b : quotation_of F.cardinal_inv_2b.
+  #[export] Declare Instance qEqual_cardinal : quotation_of F.Equal_cardinal.
+  #[export] Declare Instance qcardinal_m : quotation_of F.cardinal_m.
+  #[export] Declare Instance qempty_cardinal : quotation_of F.empty_cardinal.
+  #[export] Declare Instance qsingleton_cardinal : quotation_of F.singleton_cardinal.
+  #[export] Declare Instance qdiff_inter_cardinal : quotation_of F.diff_inter_cardinal.
+  #[export] Declare Instance qunion_cardinal : quotation_of F.union_cardinal.
+  #[export] Declare Instance qsubset_cardinal : quotation_of F.subset_cardinal.
+  #[export] Declare Instance qsubset_cardinal_lt : quotation_of F.subset_cardinal_lt.
+  #[export] Declare Instance qunion_inter_cardinal : quotation_of F.union_inter_cardinal.
+  #[export] Declare Instance qunion_cardinal_inter : quotation_of F.union_cardinal_inter.
+  #[export] Declare Instance qunion_cardinal_le : quotation_of F.union_cardinal_le.
+  #[export] Declare Instance qadd_cardinal_1 : quotation_of F.add_cardinal_1.
+  #[export] Declare Instance qadd_cardinal_2 : quotation_of F.add_cardinal_2.
+  #[export] Declare Instance qremove_cardinal_1 : quotation_of F.remove_cardinal_1.
+  #[export] Declare Instance qremove_cardinal_2 : quotation_of F.remove_cardinal_2.
+End QuotationOfWPropertiesOn.
 
-Module Type QuotationOfHasOrdOps (T : TypElt) (S : HasOrdOps T).
-  #[export] Declare Instance qcompare : quotation_of S.compare.
-  #[export] Declare Instance qmin_elt : quotation_of S.min_elt.
-  #[export] Declare Instance qmax_elt : quotation_of S.max_elt.
-End QuotationOfHasOrdOps.
+Module Type QuotationOfWProperties (M : WSets) (F : WPropertiesSig M) := QuotationOfWPropertiesOn M.E M F.
 
-Module Type QuotationOfSetsOn (E : Orders.OrderedType) (W : SetsOn E).
-  Include QuotationOfWSetsOn E W <+ QuotationOfHasOrdOps W W <+ QuotationOfHasLt W W <+ QuotationOfIsStrOrder W W.
-  #[export] Declare Instance qcompare_spec : quotation_of W.compare_spec.
-  #[export] Declare Instance qelements_spec2 : quotation_of W.elements_spec2.
-  #[export] Declare Instance qmin_elt_spec1 : quotation_of W.min_elt_spec1.
-  #[export] Declare Instance qmin_elt_spec2 : quotation_of W.min_elt_spec2.
-  #[export] Declare Instance qmin_elt_spec3 : quotation_of W.min_elt_spec3.
-  #[export] Declare Instance qmax_elt_spec1 : quotation_of W.max_elt_spec1.
-  #[export] Declare Instance qmax_elt_spec2 : quotation_of W.max_elt_spec2.
-  #[export] Declare Instance qmax_elt_spec3 : quotation_of W.max_elt_spec3.
-  #[export] Declare Instance qchoose_spec3 : quotation_of W.choose_spec3.
-End QuotationOfSetsOn.
+Module Type QuotationOfOrdProperties (M : Sets) (F : OrdPropertiesSig M) (qE : QuotationOfOrderedType M.E).
+  Module qME := QuotationOfOrderedTypeFacts M.E F.ME qE.
+  (*Module qML := QuotationOfOrderedTypeLists M.E F.ML.*)
+  Module qP := Nop <+ QuotationOfWProperties M F.P.
+  Export (hints) qME (*qML*) qP.
+  #[export] Declare Instance qsort_equivlistA_eqlistA : quotation_of F.sort_equivlistA_eqlistA.
+  #[export] Declare Instance qgtb : quotation_of F.gtb.
+  #[export] Declare Instance qleb : quotation_of F.leb.
+  #[export] Declare Instance qelements_lt : quotation_of F.elements_lt.
+  #[export] Declare Instance qelements_ge : quotation_of F.elements_ge.
+  #[export] Declare Instance qgtb_1 : quotation_of F.gtb_1.
+  #[export] Declare Instance qleb_1 : quotation_of F.leb_1.
+  #[export] Declare Instance qgtb_compat : quotation_of F.gtb_compat.
+  #[export] Declare Instance qleb_compat : quotation_of F.leb_compat.
+  #[export] Declare Instance qelements_split : quotation_of F.elements_split.
+  #[export] Declare Instance qelements_Add : quotation_of F.elements_Add.
+  #[export] Declare Instance qAbove : quotation_of F.Above.
+  #[export] Declare Instance qBelow : quotation_of F.Below.
+  #[export] Declare Instance qelements_Add_Above : quotation_of F.elements_Add_Above.
+  #[export] Declare Instance qelements_Add_Below : quotation_of F.elements_Add_Below.
+  #[export] Declare Instance qset_induction_max : quotation_of F.set_induction_max.
+  #[export] Declare Instance qset_induction_min : quotation_of F.set_induction_min.
+  #[export] Declare Instance qfold_3 : quotation_of F.fold_3.
+  #[export] Declare Instance qfold_4 : quotation_of F.fold_4.
+  #[export] Declare Instance qfold_equal : quotation_of F.fold_equal.
+  #[export] Declare Instance qadd_fold : quotation_of F.add_fold.
+  #[export] Declare Instance qremove_fold_2 : quotation_of F.remove_fold_2.
+  #[export] Declare Instance qchoose_equal : quotation_of F.choose_equal.
+End QuotationOfOrdProperties.
 
-Module ExtraQuotationOfSetsOn (M : Sets) (qE : QuotationOfOrderedType M.E) (Import qM : QuotationOfSetsOn M.E M).
-  Include ExtraQuotationOfWSetsOn M.E M qE qM.
-  Import (hints) qE qM.
-
-  Module QuotationOfOrdProperties (O : OrdPropertiesSig M).
-    Module qME := QuotationOfOrderedTypeFacts M.E O.ME qE.
-    Export (hints) qME.
-    (*Module Import ML:=OrderedTypeLists(M.E).*)
-    Module qP := QuotationOfWPropertiesOn O.P.
-    Export (hints) qP.
-    #[export] Instance qsort_equivlistA_eqlistA : quotation_of O.sort_equivlistA_eqlistA := ltac:(unfold_quotation_of (); exact _).
-    #[export] Instance qgtb : quotation_of O.gtb := ltac:(unfold_quotation_of (); exact _).
-    #[export] Instance qleb : quotation_of O.leb := ltac:(unfold_quotation_of (); exact _).
-    #[export] Instance qelements_lt : quotation_of O.elements_lt := ltac:(unfold_quotation_of (); exact _).
-    #[export] Instance qelements_ge : quotation_of O.elements_ge := ltac:(unfold_quotation_of (); exact _).
-    (*
-    #[export] Instance qgtb_1 : quotation_of O.gtb_1 := ltac:(unfold_quotation_of (); exact _).
-    #[export] Instance qleb_1 : quotation_of O.leb_1 := ltac:(unfold_quotation_of (); exact _).
-    #[export] Instance qgtb_compat : quotation_of O.gtb_compat := ltac:(unfold_quotation_of (); exact _).
-    #[export] Instance qleb_compat : quotation_of O.leb_compat := ltac:(unfold_quotation_of (); exact _).
-    #[export] Instance qelements_split : quotation_of O.elements_split := ltac:(unfold_quotation_of (); exact _).
-    #[export] Instance qelements_Add : quotation_of O.elements_Add := ltac:(unfold_quotation_of (); exact _).*)
-    #[export] Instance qAbove : quotation_of O.Above := ltac:(unfold_quotation_of (); exact _).
-    #[export] Instance qBelow : quotation_of O.Below := ltac:(unfold_quotation_of (); exact _).
-    (*#[export] Instance qelements_Add_Above : quotation_of O.elements_Add_Above := ltac:(unfold_quotation_of (); exact _).
-    #[export] Instance qelements_Add_Below : quotation_of O.elements_Add_Below := ltac:(unfold_quotation_of (); exact _).
-    #[export] Instance qset_induction_max : quotation_of O.set_induction_max := ltac:(unfold_quotation_of (); exact _).
-    #[export] Instance qset_induction_min : quotation_of O.set_induction_min := ltac:(unfold_quotation_of (); exact _).
-    #[export] Instance qfold_3 : quotation_of O.fold_3 := ltac:(unfold_quotation_of (); exact _).
-    #[export] Instance qfold_4 : quotation_of O.fold_4 := ltac:(unfold_quotation_of (); exact _).
-    #[export] Instance qfold_equal : quotation_of O.fold_equal := ltac:(unfold_quotation_of (); exact _).
-    #[export] Instance qadd_fold : quotation_of O.add_fold := ltac:(unfold_quotation_of (); exact _).
-    #[export] Instance qremove_fold_2 : quotation_of O.remove_fold_2 := ltac:(unfold_quotation_of (); exact _).
-    #[export] Instance qchoose_equal : quotation_of O.choose_equal := ltac:(unfold_quotation_of (); exact _).*)
-  End QuotationOfOrdProperties.
-End ExtraQuotationOfSetsOn.
-
-Module QuoteWSetsOn (E : DecidableType) (Import W : WSetsOn E) (qE : QuotationOfDecidableType E) (qW : QuotationOfWSetsOn E W).
+Module QuoteWSetsOn (E : DecidableType) (Import W : WSetsOn E) (WProperties : WPropertiesOnSig E W) (qE : QuotationOfDecidableType E) (qW : QuotationOfWSetsOn E W) (qWProperties : QuotationOfWPropertiesOn E W WProperties).
   Export (hints) qE.
   Export (hints) qW.
+  Export (hints) qWProperties.
+  (*
   Module qW' := ExtraQuotationOfWSetsOn E W qE qW.
   Export (hints) qW'.
   Module WFacts := WFactsOn E W.
@@ -391,6 +372,14 @@ Module QuoteWSetsOn (E : DecidableType) (Import W : WSetsOn E) (qE : QuotationOf
   Module qWProperties := qW'.QuotationOfWPropertiesOn WProperties.
   Module qWDecide := qW'.QuotationOfWDecideOn WDecide.
   Export (hints) qWFacts qWProperties qWDecide.
+   *)
+  #[export] Instance qelt : quotation_of W.elt := ltac:(unfold_quotation_of (); exact _).
+  #[export] Instance qEqual : quotation_of W.Equal := ltac:(unfold_quotation_of (); exact _).
+  #[export] Instance qSubset : quotation_of W.Subset := ltac:(unfold_quotation_of (); exact _).
+  #[export] Instance qEmpty : quotation_of W.Empty := ltac:(unfold_quotation_of (); exact _).
+  #[export] Instance qFor_all : quotation_of W.For_all := ltac:(unfold_quotation_of (); exact _).
+  #[export] Instance qExists : quotation_of W.Exists := ltac:(unfold_quotation_of (); exact _).
+  #[export] Instance qeq : quotation_of W.eq := ltac:(unfold_quotation_of (); exact _).
 
   #[export] Instance quote_In {x y} {qx : quotation_of x} {qy : quotation_of y} : ground_quotable (In x y)
     := ground_quotable_of_dec (WProperties.In_dec x y).
@@ -415,7 +404,7 @@ Module QuoteWSetsOn (E : DecidableType) (Import W : WSetsOn E) (qE : QuotationOf
     : For_all_alt P s <-> For_all P s.
   Proof using Type.
     cbv [For_all_alt For_all].
-    setoid_rewrite WFacts.elements_iff.
+    setoid_rewrite WProperties.FM.elements_iff.
     induction (elements s) as [|x xs IH].
     { split; solve [ constructor | inversion 2 ]. }
     { setoid_rewrite Forall_cons_iff; setoid_rewrite InA_cons; setoid_rewrite IH.
@@ -441,7 +430,7 @@ Module QuoteWSetsOn (E : DecidableType) (Import W : WSetsOn E) (qE : QuotationOf
     : Exists_alt P s <-> Exists P s.
   Proof.
     cbv [Exists_alt Exists].
-    setoid_rewrite WFacts.elements_iff.
+    setoid_rewrite WProperties.FM.elements_iff.
     induction (elements s) as [|x xs IH].
     { split; try solve [ constructor | inversion 1 | intros [x [H H']]; inversion H ]. }
     { setoid_rewrite Exists_cons; setoid_rewrite InA_cons; setoid_rewrite IH.
@@ -464,14 +453,9 @@ Module QuoteWSetsOn (E : DecidableType) (Import W : WSetsOn E) (qE : QuotationOf
   => simple notypeclasses refine (@quote_For_all _ _ _ _ _ _ _ _ _ _ _ _ _ _ _ _) : typeclass_instances.
 End QuoteWSetsOn.
 
-Module QuoteSetsOn (E : OrderedType) (Import M : SetsOn E) (qE : QuotationOfOrderedType E) (qM : QuotationOfSetsOn E M).
-  Module Import QuoteSetsOnInner := QuoteWSetsOn E M qE qM.
-  Export (hints) qE.
-  Export (hints) QuoteSetsOnInner.
-  Module Import MOrdProperties. Module E := E. Include M <+ OrdProperties. End MOrdProperties.
-  Module Import qM := ExtraQuotationOfSetsOn MOrdProperties qE qM.
-  Module qMOrdProperties := qM.QuotationOfOrdProperties MOrdProperties.
-  Export (hints) qMOrdProperties.
+Module QuoteSets (Import M : Sets) (Import MOrdProperties : OrdPropertiesSig M) (qE : QuotationOfOrderedType M.E) (qM : QuotationOfSets M) (qMOrdProperties : QuotationOfOrdProperties M MOrdProperties qE).
+  Export (hints) qE qM qMOrdProperties.
+  Include QuoteWSetsOn M.E M MOrdProperties.P qE qM qMOrdProperties.qP.
 
   Definition above x s : bool := for_all (fun y => if ME.lt_dec y x then true else false) s.
   Definition below x s : bool := for_all (fun y => if ME.lt_dec x y then true else false) s.
@@ -501,309 +485,476 @@ Module QuoteSetsOn (E : OrderedType) (Import M : SetsOn E) (qE : QuotationOfOrde
     := ground_quotable_of_iff (above_spec x s).
   #[export] Instance quote_Below {x s} {qx : quotation_of x} {qs : quotation_of s} : ground_quotable (Below x s)
     := ground_quotable_of_iff (below_spec x s).
-End QuoteSetsOn.
+End QuoteSets.
 
-Module MSetAVL.
-  Module Type MakeSig (T : OrderedType) := Nop <+ MSetAVL.Make T.
-  Module Type QuotationOfMake (T : OrderedType) (M : MakeSig T) (qT : QuotationOfOrderedType T).
-    #[export] Declare Instance qt_ : inductive_quotation_of M.t_.
-    #[export] Declare Instance qRaw_enumeration : inductive_quotation_of M.Raw.enumeration.
-    #[export] Declare Instance qRaw_tree : inductive_quotation_of M.Raw.tree.
-    #[export] Declare Instance qRaw_bst : inductive_quotation_of M.Raw.bst.
-    #[export] Declare Instance qRaw_InT : inductive_quotation_of M.Raw.InT.
-    #[export] Declare Instance qRaw_R_min_elt : inductive_quotation_of M.Raw.R_min_elt.
-    #[export] Declare Instance qRaw_R_max_elt : inductive_quotation_of M.Raw.R_max_elt.
-    #[export] Declare Instance qRaw_R_bal : inductive_quotation_of M.Raw.R_bal.
-    #[export] Declare Instance qRaw_R_remove_min : inductive_quotation_of M.Raw.R_remove_min.
-    #[export] Declare Instance qRaw_R_merge : inductive_quotation_of M.Raw.R_merge.
-    #[export] Declare Instance qRaw_R_concat : inductive_quotation_of M.Raw.R_concat.
-    #[export] Declare Instance qRaw_R_inter : inductive_quotation_of M.Raw.R_inter.
-    #[export] Declare Instance qRaw_R_diff : inductive_quotation_of M.Raw.R_diff.
-    #[export] Declare Instance qRaw_R_union : inductive_quotation_of M.Raw.R_union.
-    #[export] Declare Instance qRaw_triple : inductive_quotation_of M.Raw.triple.
-  End QuotationOfMake.
+Module Export MSets.
+  Module MSetAVL.
+    Module Type MakeSig (T : OrderedType) := Nop <+ MSetAVL.Make T.
+    Module Type QuotationOfMake (T : OrderedType) (M : MakeSig T).
+      Module qRaw.
+        #[export] Declare Instance qelt : quotation_of M.Raw.elt.
+        #[export] Declare Instance qtree : inductive_quotation_of M.Raw.tree.
+        #[export] Declare Instance qempty : quotation_of M.Raw.empty.
+        #[export] Declare Instance qis_empty : quotation_of M.Raw.is_empty.
+        #[export] Declare Instance qmem : quotation_of M.Raw.mem.
+        #[export] Declare Instance qmin_elt : quotation_of M.Raw.min_elt.
+        #[export] Declare Instance qmax_elt : quotation_of M.Raw.max_elt.
+        #[export] Declare Instance qchoose : quotation_of M.Raw.choose.
+        #[export] Declare Instance qfold : quotation_of (@M.Raw.fold).
+        #[export] Declare Instance qelements_aux : quotation_of M.Raw.elements_aux.
+        #[export] Declare Instance qelements : quotation_of M.Raw.elements.
+        #[export] Declare Instance qrev_elements_aux : quotation_of M.Raw.rev_elements_aux.
+        #[export] Declare Instance qrev_elements : quotation_of M.Raw.rev_elements.
+        #[export] Declare Instance qcardinal : quotation_of M.Raw.cardinal.
+        #[export] Declare Instance qmaxdepth : quotation_of M.Raw.maxdepth.
+        #[export] Declare Instance qmindepth : quotation_of M.Raw.mindepth.
+        #[export] Declare Instance qfor_all : quotation_of M.Raw.for_all.
+        #[export] Declare Instance qexists_ : quotation_of M.Raw.exists_.
+        #[export] Declare Instance qenumeration : inductive_quotation_of M.Raw.enumeration.
+        #[export] Declare Instance qcons : quotation_of M.Raw.cons.
+        #[export] Declare Instance qcompare_more : quotation_of M.Raw.compare_more.
+        #[export] Declare Instance qcompare_cont : quotation_of M.Raw.compare_cont.
+        #[export] Declare Instance qcompare_end : quotation_of M.Raw.compare_end.
+        #[export] Declare Instance qcompare : quotation_of M.Raw.compare.
+        #[export] Declare Instance qequal : quotation_of M.Raw.equal.
+        #[export] Declare Instance qsubsetl : quotation_of M.Raw.subsetl.
+        #[export] Declare Instance qsubsetr : quotation_of M.Raw.subsetr.
+        #[export] Declare Instance qsubset : quotation_of M.Raw.subset.
+        #[export] Declare Instance qheight : quotation_of M.Raw.height.
+        #[export] Declare Instance qsingleton : quotation_of M.Raw.singleton.
+        #[export] Declare Instance qcreate : quotation_of M.Raw.create.
+        #[export] Declare Instance qassert_false : quotation_of M.Raw.assert_false.
+        #[export] Declare Instance qbal : quotation_of M.Raw.bal.
+        #[export] Declare Instance qadd : quotation_of M.Raw.add.
+        #[export] Declare Instance qjoin : quotation_of M.Raw.join.
+        #[export] Declare Instance qremove_min : quotation_of M.Raw.remove_min.
+        #[export] Declare Instance qmerge : quotation_of M.Raw.merge.
+        #[export] Declare Instance qremove : quotation_of M.Raw.remove.
+        #[export] Declare Instance qconcat : quotation_of M.Raw.concat.
+        #[export] Declare Instance qt_left : quotation_of M.Raw.t_left.
+        #[export] Declare Instance qt_in : quotation_of M.Raw.t_in.
+        #[export] Declare Instance qt_right : quotation_of M.Raw.t_right.
+        #[export] Declare Instance qsplit : quotation_of M.Raw.split.
+        #[export] Declare Instance qinter : quotation_of M.Raw.inter.
+        #[export] Declare Instance qdiff : quotation_of M.Raw.diff.
+        #[export] Declare Instance qunion : quotation_of M.Raw.union.
+        #[export] Declare Instance qfilter : quotation_of M.Raw.filter.
+        #[export] Declare Instance qpartition : quotation_of M.Raw.partition.
+        #[export] Declare Instance qInT : inductive_quotation_of M.Raw.InT.
+        #[export] Declare Instance qIn : quotation_of M.Raw.In.
+        #[export] Declare Instance qEqual : quotation_of M.Raw.Equal.
+        #[export] Declare Instance qSubset : quotation_of M.Raw.Subset.
+        #[export] Declare Instance qEmpty : quotation_of M.Raw.Empty.
+        #[export] Declare Instance qFor_all : quotation_of M.Raw.For_all.
+        #[export] Declare Instance qExists : quotation_of M.Raw.Exists.
+        #[export] Declare Instance qlt_tree : quotation_of M.Raw.lt_tree.
+        #[export] Declare Instance qgt_tree : quotation_of M.Raw.gt_tree.
+        #[export] Declare Instance qbst : inductive_quotation_of M.Raw.bst.
+        #[export] Declare Instance qIsOk : quotation_of M.Raw.IsOk.
+        #[export] Declare Instance qOk : quotation_of M.Raw.Ok.
+        #[export] Declare Instance qok : quotation_of (@M.Raw.ok).
+        #[export] Declare Instance qbst_Ok : quotation_of M.Raw.bst_Ok.
+        #[export] Declare Instance qltb_tree : quotation_of M.Raw.ltb_tree.
+        #[export] Declare Instance qgtb_tree : quotation_of M.Raw.gtb_tree.
+        #[export] Declare Instance qisok : quotation_of M.Raw.isok.
+        #[export] Declare Instance qltb_tree_iff : quotation_of M.Raw.ltb_tree_iff.
+        #[export] Declare Instance qgtb_tree_iff : quotation_of M.Raw.gtb_tree_iff.
+        #[export] Declare Instance qisok_iff : quotation_of M.Raw.isok_iff.
+        #[export] Declare Instance qisok_Ok : quotation_of M.Raw.isok_Ok.
+        #[export] Declare Instance qIn_1 : quotation_of M.Raw.In_1.
+        #[export] Declare Instance qIn_compat : quotation_of M.Raw.In_compat.
+        #[export] Declare Instance qIn_node_iff : quotation_of M.Raw.In_node_iff.
+        #[export] Declare Instance qIn_leaf_iff : quotation_of M.Raw.In_leaf_iff.
+        #[export] Declare Instance qlt_leaf : quotation_of M.Raw.lt_leaf.
+        #[export] Declare Instance qgt_leaf : quotation_of M.Raw.gt_leaf.
+        #[export] Declare Instance qlt_tree_node : quotation_of M.Raw.lt_tree_node.
+        #[export] Declare Instance qgt_tree_node : quotation_of M.Raw.gt_tree_node.
+        #[export] Declare Instance qlt_tree_not_in : quotation_of M.Raw.lt_tree_not_in.
+        #[export] Declare Instance qlt_tree_trans : quotation_of M.Raw.lt_tree_trans.
+        #[export] Declare Instance qgt_tree_not_in : quotation_of M.Raw.gt_tree_not_in.
+        #[export] Declare Instance qgt_tree_trans : quotation_of M.Raw.gt_tree_trans.
+        #[export] Declare Instance qlt_tree_compat : quotation_of M.Raw.lt_tree_compat.
+        #[export] Declare Instance qgt_tree_compat : quotation_of M.Raw.gt_tree_compat.
+        #[export] Declare Instance qempty_spec : quotation_of M.Raw.empty_spec.
+        #[export] Declare Instance qempty_ok : quotation_of M.Raw.empty_ok.
+        #[export] Declare Instance qis_empty_spec : quotation_of M.Raw.is_empty_spec.
+        #[export] Declare Instance qmem_spec : quotation_of M.Raw.mem_spec.
+        #[export] Declare Instance qR_min_elt : inductive_quotation_of M.Raw.R_min_elt.
+        #[export] Declare Instance qmin_elt_equation : quotation_of M.Raw.min_elt_equation.
+        #[export] Declare Instance qR_max_elt : inductive_quotation_of M.Raw.R_max_elt.
+        #[export] Declare Instance qmax_elt_equation : quotation_of M.Raw.max_elt_equation.
+        #[export] Declare Instance qmin_elt_spec1 : quotation_of M.Raw.min_elt_spec1.
+        #[export] Declare Instance qmin_elt_spec2 : quotation_of M.Raw.min_elt_spec2.
+        #[export] Declare Instance qmin_elt_spec3 : quotation_of M.Raw.min_elt_spec3.
+        #[export] Declare Instance qmax_elt_spec1 : quotation_of M.Raw.max_elt_spec1.
+        #[export] Declare Instance qmax_elt_spec2 : quotation_of M.Raw.max_elt_spec2.
+        #[export] Declare Instance qmax_elt_spec3 : quotation_of M.Raw.max_elt_spec3.
+        #[export] Declare Instance qchoose_spec1 : quotation_of M.Raw.choose_spec1.
+        #[export] Declare Instance qchoose_spec2 : quotation_of M.Raw.choose_spec2.
+        #[export] Declare Instance qchoose_spec3 : quotation_of M.Raw.choose_spec3.
+        #[export] Declare Instance qelements_spec1' : quotation_of M.Raw.elements_spec1'.
+        #[export] Declare Instance qelements_spec1 : quotation_of M.Raw.elements_spec1.
+        #[export] Declare Instance qelements_spec2' : quotation_of M.Raw.elements_spec2'.
+        #[export] Declare Instance qelements_spec2 : quotation_of M.Raw.elements_spec2.
+        #[export] Declare Instance qelements_spec2w : quotation_of M.Raw.elements_spec2w.
+        #[export] Declare Instance qelements_aux_cardinal : quotation_of M.Raw.elements_aux_cardinal.
+        #[export] Declare Instance qelements_cardinal : quotation_of M.Raw.elements_cardinal.
+        #[export] Declare Instance qcardinal_spec : quotation_of M.Raw.cardinal_spec.
+        #[export] Declare Instance qelements_app : quotation_of M.Raw.elements_app.
+        #[export] Declare Instance qelements_node : quotation_of M.Raw.elements_node.
+        #[export] Declare Instance qrev_elements_app : quotation_of M.Raw.rev_elements_app.
+        #[export] Declare Instance qrev_elements_node : quotation_of M.Raw.rev_elements_node.
+        #[export] Declare Instance qrev_elements_rev : quotation_of M.Raw.rev_elements_rev.
+        #[export] Declare Instance qsorted_app_inv : quotation_of M.Raw.sorted_app_inv.
+        #[export] Declare Instance qelements_sort_ok : quotation_of M.Raw.elements_sort_ok.
+        #[export] Declare Instance qfor_all_spec : quotation_of M.Raw.for_all_spec.
+        #[export] Declare Instance qexists_spec : quotation_of M.Raw.exists_spec.
+        #[export] Declare Instance qfold_spec' : quotation_of (@M.Raw.fold_spec').
+        #[export] Declare Instance qfold_spec : quotation_of M.Raw.fold_spec.
+        #[export] Declare Instance qsubsetl_spec : quotation_of M.Raw.subsetl_spec.
+        #[export] Declare Instance qsubsetr_spec : quotation_of M.Raw.subsetr_spec.
+        #[export] Declare Instance qsubset_spec : quotation_of M.Raw.subset_spec.
+        #[export] Declare Instance qeq : quotation_of M.Raw.eq.
+        #[export] Declare Instance qeq_equiv : quotation_of M.Raw.eq_equiv.
+        #[export] Declare Instance qeq_Leq : quotation_of M.Raw.eq_Leq.
+        #[export] Declare Instance qlt : quotation_of M.Raw.lt.
+        #[export] Declare Instance qlt_strorder : quotation_of M.Raw.lt_strorder.
+        #[export] Declare Instance qlt_compat : quotation_of M.Raw.lt_compat.
+        #[export] Declare Instance qflatten_e : quotation_of M.Raw.flatten_e.
+        #[export] Declare Instance qflatten_e_elements : quotation_of M.Raw.flatten_e_elements.
+        #[export] Declare Instance qcons_1 : quotation_of M.Raw.cons_1.
+        #[export] Declare Instance qCmp : quotation_of M.Raw.Cmp.
+        #[export] Declare Instance qcompare_end_Cmp : quotation_of M.Raw.compare_end_Cmp.
+        #[export] Declare Instance qcompare_more_Cmp : quotation_of M.Raw.compare_more_Cmp.
+        #[export] Declare Instance qcompare_cont_Cmp : quotation_of M.Raw.compare_cont_Cmp.
+        #[export] Declare Instance qcompare_Cmp : quotation_of M.Raw.compare_Cmp.
+        #[export] Declare Instance qcompare_spec : quotation_of M.Raw.compare_spec.
+        #[export] Declare Instance qequal_spec : quotation_of M.Raw.equal_spec.
+        #[export] Declare Instance qmindepth_maxdepth : quotation_of M.Raw.mindepth_maxdepth.
+        #[export] Declare Instance qmaxdepth_cardinal : quotation_of M.Raw.maxdepth_cardinal.
+        #[export] Declare Instance qmindepth_cardinal : quotation_of M.Raw.mindepth_cardinal.
+        #[export] Declare Instance qmaxdepth_log_cardinal : quotation_of M.Raw.maxdepth_log_cardinal.
+        #[export] Declare Instance qmindepth_log_cardinal : quotation_of M.Raw.mindepth_log_cardinal.
+        #[export] Declare Instance qR_bal : inductive_quotation_of M.Raw.R_bal.
+        #[export] Declare Instance qR_remove_min : inductive_quotation_of M.Raw.R_remove_min.
+        #[export] Declare Instance qremove_min_equation : quotation_of M.Raw.remove_min_equation.
+        #[export] Declare Instance qR_merge : inductive_quotation_of M.Raw.R_merge.
+        #[export] Declare Instance qR_concat : inductive_quotation_of M.Raw.R_concat.
+        #[export] Declare Instance qR_inter : inductive_quotation_of M.Raw.R_inter.
+        #[export] Declare Instance qinter_equation : quotation_of M.Raw.inter_equation.
+        #[export] Declare Instance qR_diff : inductive_quotation_of M.Raw.R_diff.
+        #[export] Declare Instance qdiff_equation : quotation_of M.Raw.diff_equation.
+        #[export] Declare Instance qR_union : inductive_quotation_of M.Raw.R_union.
+        #[export] Declare Instance qunion_equation : quotation_of M.Raw.union_equation.
+        #[export] Declare Instance qsingleton_spec : quotation_of M.Raw.singleton_spec.
+        #[export] Declare Instance qsingleton_ok : quotation_of M.Raw.singleton_ok.
+        #[export] Declare Instance qcreate_spec : quotation_of M.Raw.create_spec.
+        #[export] Declare Instance qcreate_ok : quotation_of M.Raw.create_ok.
+        #[export] Declare Instance qbal_spec : quotation_of M.Raw.bal_spec.
+        #[export] Declare Instance qbal_ok : quotation_of M.Raw.bal_ok.
+        #[export] Declare Instance qadd_spec' : quotation_of M.Raw.add_spec'.
+        #[export] Declare Instance qadd_spec : quotation_of M.Raw.add_spec.
+        #[export] Declare Instance qadd_ok : quotation_of M.Raw.add_ok.
+        #[export] Declare Instance qjoin_spec : quotation_of M.Raw.join_spec.
+        #[export] Declare Instance qjoin_ok : quotation_of M.Raw.join_ok.
+        #[export] Declare Instance qremove_min_spec : quotation_of M.Raw.remove_min_spec.
+        #[export] Declare Instance qremove_min_ok : quotation_of M.Raw.remove_min_ok.
+        #[export] Declare Instance qremove_min_gt_tree : quotation_of M.Raw.remove_min_gt_tree.
+        #[export] Declare Instance qmerge_spec : quotation_of M.Raw.merge_spec.
+        #[export] Declare Instance qmerge_ok : quotation_of M.Raw.merge_ok.
+        #[export] Declare Instance qremove_spec : quotation_of M.Raw.remove_spec.
+        #[export] Declare Instance qremove_ok : quotation_of M.Raw.remove_ok.
+        #[export] Declare Instance qconcat_spec : quotation_of M.Raw.concat_spec.
+        #[export] Declare Instance qconcat_ok : quotation_of M.Raw.concat_ok.
+        #[export] Declare Instance qsplit_spec1 : quotation_of M.Raw.split_spec1.
+        #[export] Declare Instance qsplit_spec2 : quotation_of M.Raw.split_spec2.
+        #[export] Declare Instance qsplit_spec3 : quotation_of M.Raw.split_spec3.
+        #[export] Declare Instance qsplit_ok : quotation_of M.Raw.split_ok.
+        #[export] Declare Instance qsplit_ok1 : quotation_of M.Raw.split_ok1.
+        #[export] Declare Instance qsplit_ok2 : quotation_of M.Raw.split_ok2.
+        #[export] Declare Instance qinter_spec_ok : quotation_of (@M.Raw.inter_spec_ok).
+        #[export] Declare Instance qinter_spec : quotation_of M.Raw.inter_spec.
+        #[export] Declare Instance qinter_ok : quotation_of M.Raw.inter_ok.
+        #[export] Declare Instance qdiff_spec_ok : quotation_of (@M.Raw.diff_spec_ok).
+        #[export] Declare Instance qdiff_spec : quotation_of M.Raw.diff_spec.
+        #[export] Declare Instance qdiff_ok : quotation_of M.Raw.diff_ok.
+        #[export] Declare Instance qunion_spec : quotation_of M.Raw.union_spec.
+        #[export] Declare Instance qunion_ok : quotation_of M.Raw.union_ok.
+        #[export] Declare Instance qfilter_spec : quotation_of M.Raw.filter_spec.
+        #[export] Declare Instance qfilter_weak_spec : quotation_of M.Raw.filter_weak_spec.
+        #[export] Declare Instance qfilter_ok : quotation_of M.Raw.filter_ok.
+        #[export] Declare Instance qpartition_spec1' : quotation_of M.Raw.partition_spec1'.
+        #[export] Declare Instance qpartition_spec2' : quotation_of M.Raw.partition_spec2'.
+        #[export] Declare Instance qpartition_spec1 : quotation_of M.Raw.partition_spec1.
+        #[export] Declare Instance qpartition_spec2 : quotation_of M.Raw.partition_spec2.
+        #[export] Declare Instance qpartition_ok1 : quotation_of M.Raw.partition_ok1.
+        #[export] Declare Instance qpartition_ok2 : quotation_of M.Raw.partition_ok2.
+      End qRaw.
+      Export (hints) qRaw.
 
-  Module ExtraQuotationOfMake (T : OrderedType) (M : MakeSig T) (Import qT : QuotationOfOrderedType T) (Import qM : QuotationOfMake T M qT) <: QuotationOfWSetsOn T M.
-    Module Raw.
-      Module qMX := QuotationOfOrderedTypeFacts T M.Raw.MX qT.
-      Export (hints) qMX.
-      #[export] Instance qelt : quotation_of M.Raw.elt := ltac:(unfold_quotation_of (); exact _).
-      #[export] Instance qtree_ind : quotation_of M.Raw.tree_ind := ltac:(unfold_quotation_of (); exact _).
-      #[export] Instance qempty : quotation_of M.Raw.empty := ltac:(unfold_quotation_of (); exact _).
-      #[export] Instance qis_empty : quotation_of M.Raw.is_empty := ltac:(unfold_quotation_of (); exact _).
-      #[export] Instance qmem : quotation_of M.Raw.mem := ltac:(unfold_quotation_of (); exact _).
-      #[export] Instance qmin_elt : quotation_of M.Raw.min_elt := ltac:(unfold_quotation_of (); exact _).
-      #[export] Instance qmax_elt : quotation_of M.Raw.max_elt := ltac:(unfold_quotation_of (); exact _).
-      #[export] Instance qchoose : quotation_of M.Raw.choose := ltac:(unfold_quotation_of (); exact _).
-      #[export] Instance qfold : quotation_of (@M.Raw.fold) := ltac:(unfold_quotation_of (); exact _).
-      #[export] Instance qelements_aux : quotation_of M.Raw.elements_aux := ltac:(unfold_quotation_of (); exact _).
-      #[export] Instance qelements : quotation_of M.Raw.elements := ltac:(unfold_quotation_of (); exact _).
-      #[export] Instance qrev_elements_aux : quotation_of M.Raw.rev_elements_aux := ltac:(unfold_quotation_of (); exact _).
-      #[export] Instance qrev_elements : quotation_of M.Raw.rev_elements := ltac:(unfold_quotation_of (); exact _).
-      #[export] Instance qcardinal : quotation_of M.Raw.cardinal := ltac:(unfold_quotation_of (); exact _).
-      #[export] Instance qmaxdepth : quotation_of M.Raw.maxdepth := ltac:(unfold_quotation_of (); exact _).
-      #[export] Instance qmindepth : quotation_of M.Raw.mindepth := ltac:(unfold_quotation_of (); exact _).
-      #[export] Instance qfor_all : quotation_of M.Raw.for_all := ltac:(unfold_quotation_of (); exact _).
-      #[export] Instance qexists_ : quotation_of M.Raw.exists_ := ltac:(unfold_quotation_of (); exact _).
-      #[export] Instance qcons : quotation_of M.Raw.cons := ltac:(unfold_quotation_of (); exact _).
-      #[export] Instance qcompare_more : quotation_of M.Raw.compare_more := ltac:(unfold_quotation_of (); exact _).
-      Print M.Raw.
+      #[export] Declare Instance qelt : quotation_of M.elt.
+      #[export] Declare Instance qt_ : inductive_quotation_of M.t_.
+      #[export] Declare Instance qthis : quotation_of M.this.
+      #[export] Declare Instance qis_ok : quotation_of M.is_ok.
+      #[export] Declare Instance qt : quotation_of M.t.
+      #[export] Declare Instance qIn : quotation_of M.In.
+      #[export] Declare Instance qEqual : quotation_of M.Equal.
+      #[export] Declare Instance qSubset : quotation_of M.Subset.
+      #[export] Declare Instance qEmpty : quotation_of M.Empty.
+      #[export] Declare Instance qFor_all : quotation_of M.For_all.
+      #[export] Declare Instance qExists : quotation_of M.Exists.
+      #[export] Declare Instance qmem : quotation_of M.mem.
+      #[export] Declare Instance qadd : quotation_of M.add.
+      #[export] Declare Instance qremove : quotation_of M.remove.
+      #[export] Declare Instance qsingleton : quotation_of M.singleton.
+      #[export] Declare Instance qunion : quotation_of M.union.
+      #[export] Declare Instance qinter : quotation_of M.inter.
+      #[export] Declare Instance qdiff : quotation_of M.diff.
+      #[export] Declare Instance qequal : quotation_of M.equal.
+      #[export] Declare Instance qsubset : quotation_of M.subset.
+      #[export] Declare Instance qempty : quotation_of M.empty.
+      #[export] Declare Instance qis_empty : quotation_of M.is_empty.
+      #[export] Declare Instance qelements : quotation_of M.elements.
+      #[export] Declare Instance qchoose : quotation_of M.choose.
+      #[export] Declare Instance qfold : quotation_of M.fold.
+      #[export] Declare Instance qcardinal : quotation_of M.cardinal.
+      #[export] Declare Instance qfilter : quotation_of M.filter.
+      #[export] Declare Instance qfor_all : quotation_of M.for_all.
+      #[export] Declare Instance qexists_ : quotation_of M.exists_.
+      #[export] Declare Instance qpartition : quotation_of M.partition.
+      #[export] Declare Instance qIn_compat : quotation_of M.In_compat.
+      #[export] Declare Instance qeq : quotation_of M.eq.
+      #[export] Declare Instance qeq_equiv : quotation_of M.eq_equiv.
+      #[export] Declare Instance qeq_dec : quotation_of M.eq_dec.
+      #[export] Declare Instance qmem_spec : quotation_of M.mem_spec.
+      #[export] Declare Instance qequal_spec : quotation_of M.equal_spec.
+      #[export] Declare Instance qsubset_spec : quotation_of M.subset_spec.
+      #[export] Declare Instance qempty_spec : quotation_of M.empty_spec.
+      #[export] Declare Instance qis_empty_spec : quotation_of M.is_empty_spec.
+      #[export] Declare Instance qadd_spec : quotation_of M.add_spec.
+      #[export] Declare Instance qremove_spec : quotation_of M.remove_spec.
+      #[export] Declare Instance qsingleton_spec : quotation_of M.singleton_spec.
+      #[export] Declare Instance qunion_spec : quotation_of M.union_spec.
+      #[export] Declare Instance qinter_spec : quotation_of M.inter_spec.
+      #[export] Declare Instance qdiff_spec : quotation_of M.diff_spec.
+      #[export] Declare Instance qfold_spec : quotation_of M.fold_spec.
+      #[export] Declare Instance qcardinal_spec : quotation_of M.cardinal_spec.
+      #[export] Declare Instance qfilter_spec : quotation_of M.filter_spec.
+      #[export] Declare Instance qfor_all_spec : quotation_of M.for_all_spec.
+      #[export] Declare Instance qexists_spec : quotation_of M.exists_spec.
+      #[export] Declare Instance qpartition_spec1 : quotation_of M.partition_spec1.
+      #[export] Declare Instance qpartition_spec2 : quotation_of M.partition_spec2.
+      #[export] Declare Instance qelements_spec1 : quotation_of M.elements_spec1.
+      #[export] Declare Instance qelements_spec2w : quotation_of M.elements_spec2w.
+      #[export] Declare Instance qchoose_spec1 : quotation_of M.choose_spec1.
+      #[export] Declare Instance qchoose_spec2 : quotation_of M.choose_spec2.
+      #[export] Declare Instance qcompare : quotation_of M.compare.
+      #[export] Declare Instance qmin_elt : quotation_of M.min_elt.
+      #[export] Declare Instance qmax_elt : quotation_of M.max_elt.
+      #[export] Declare Instance qlt : quotation_of M.lt.
+      #[export] Declare Instance qlt_strorder : quotation_of M.lt_strorder.
+      #[export] Declare Instance qlt_compat : quotation_of M.lt_compat.
+      #[export] Declare Instance qcompare_spec : quotation_of M.compare_spec.
+      #[export] Declare Instance qelements_spec2 : quotation_of M.elements_spec2.
+      #[export] Declare Instance qmin_elt_spec1 : quotation_of M.min_elt_spec1.
+      #[export] Declare Instance qmin_elt_spec2 : quotation_of M.min_elt_spec2.
+      #[export] Declare Instance qmin_elt_spec3 : quotation_of M.min_elt_spec3.
+      #[export] Declare Instance qmax_elt_spec1 : quotation_of M.max_elt_spec1.
+      #[export] Declare Instance qmax_elt_spec2 : quotation_of M.max_elt_spec2.
+      #[export] Declare Instance qmax_elt_spec3 : quotation_of M.max_elt_spec3.
+      #[export] Declare Instance qchoose_spec3 : quotation_of M.choose_spec3.
+    End QuotationOfMake.
+  End MSetAVL.
 
-      #[export] Instance qcompare_cont : quotation_of M.Raw.compare_cont := ltac:(unfold_quotation_of (); exact _).
-      #[export] Instance qcompare_end : quotation_of M.Raw.compare_end := ltac:(unfold_quotation_of (); exact _).
-      #[export] Instance qcompare : quotation_of M.Raw.compare := ltac:(unfold_quotation_of (); exact _).
-      #[export] Instance qequal : quotation_of M.Raw.equal := ltac:(unfold_quotation_of (); exact _).
-      #[export] Instance qsubsetl : quotation_of M.Raw.subsetl := ltac:(unfold_quotation_of (); exact _).
-      #[export] Instance qsubsetr : quotation_of M.Raw.subsetr := ltac:(unfold_quotation_of (); exact _).
-      #[export] Instance qsubset : quotation_of M.Raw.subset := ltac:(unfold_quotation_of (); exact _).
-      #[export] Instance qt : quotation_of M.Raw.t := ltac:(unfold_quotation_of (); exact _).
-      #[export] Instance qheight : quotation_of M.Raw.height := ltac:(unfold_quotation_of (); exact _).
-      #[export] Instance qsingleton : quotation_of M.Raw.singleton := ltac:(unfold_quotation_of (); exact _).
-      #[export] Instance qcreate : quotation_of M.Raw.create := ltac:(unfold_quotation_of (); exact _).
-     #[export] Instance qassert_false : quotation_of M.Raw.assert_false := ltac:(unfold_quotation_of (); exact _).
-     #[export] Instance qbal : quotation_of M.Raw.bal := ltac:(unfold_quotation_of (); exact _).
-     #[export] Instance qadd : quotation_of M.Raw.add := ltac:(unfold_quotation_of (); exact _).
-     #[export] Instance qjoin : quotation_of M.Raw.join := ltac:(unfold_quotation_of (); exact _).
-     #[export] Instance qremove_min : quotation_of M.Raw.remove_min := ltac:(unfold_quotation_of (); exact _).
-     #[export] Instance qmerge : quotation_of M.Raw.merge := ltac:(unfold_quotation_of (); exact _).
-     #[export] Instance qremove : quotation_of M.Raw.remove := ltac:(unfold_quotation_of (); exact _).
-     #[export] Instance qconcat : quotation_of M.Raw.concat := ltac:(unfold_quotation_of (); exact _).
-     #[export] Instance qt_left : quotation_of M.Raw.t_left := ltac:(unfold_quotation_of (); exact _).
-     #[export] Instance qt_in : quotation_of M.Raw.t_in := ltac:(unfold_quotation_of (); exact _).
-     #[export] Instance qt_right : quotation_of M.Raw.t_right := ltac:(unfold_quotation_of (); exact _).
-     #[export] Instance qsplit : quotation_of M.Raw.split := ltac:(unfold_quotation_of (); exact _).
-     #[export] Instance qinter : quotation_of M.Raw.inter := ltac:(unfold_quotation_of (); exact _).
-     #[export] Instance qdiff : quotation_of M.Raw.diff := ltac:(unfold_quotation_of (); exact _).
-     #[export] Instance qunion : quotation_of M.Raw.union := ltac:(unfold_quotation_of (); exact _).
-     #[export] Instance qfilter : quotation_of M.Raw.filter := ltac:(unfold_quotation_of (); exact _).
-     #[export] Instance qpartition : quotation_of M.Raw.partition := ltac:(unfold_quotation_of (); exact _).
-     #[export] Instance qIn : quotation_of M.Raw.In := ltac:(unfold_quotation_of (); exact _).
-     #[export] Instance qEqual : quotation_of M.Raw.Equal := ltac:(unfold_quotation_of (); exact _).
-     #[export] Instance qSubset : quotation_of M.Raw.Subset := ltac:(unfold_quotation_of (); exact _).
-     #[export] Instance qEmpty : quotation_of M.Raw.Empty := ltac:(unfold_quotation_of (); exact _).
-     #[export] Instance qFor_all : quotation_of M.Raw.For_all := ltac:(unfold_quotation_of (); exact _).
-     #[export] Instance qExists : quotation_of M.Raw.Exists := ltac:(unfold_quotation_of (); exact _).
-     #[export] Instance qlt_tree : quotation_of M.Raw.lt_tree := ltac:(unfold_quotation_of (); exact _).
-     #[export] Instance qgt_tree : quotation_of M.Raw.gt_tree := ltac:(unfold_quotation_of (); exact _).
-     #[export] Instance qIsOk : quotation_of M.Raw.IsOk := ltac:(unfold_quotation_of (); exact _).
-     #[export] Instance qOk : quotation_of M.Raw.Ok := ltac:(unfold_quotation_of (); exact _).
-     #[export] Instance qok : quotation_of (@M.Raw.ok) := ltac:(unfold_quotation_of (); exact _).
-     #[export] Instance qbst_Ok : quotation_of M.Raw.bst_Ok := ltac:(unfold_quotation_of (); exact _).
-     (*
-     #[export] Instance qltb_tree : quotation_of M.Raw.ltb_tree := ltac:(unfold_quotation_of (); exact _).
-     #[export] Instance qgtb_tree : quotation_of M.Raw.gtb_tree := ltac:(unfold_quotation_of (); exact _).
-     #[export] Instance qisok : quotation_of M.Raw.isok := ltac:(unfold_quotation_of (); exact _).
-     #[export] Instance qltb_tree_iff : quotation_of M.Raw.ltb_tree_iff := ltac:(unfold_quotation_of (); exact _).
-     #[export] Instance qgtb_tree_iff : quotation_of M.Raw.gtb_tree_iff := ltac:(unfold_quotation_of (); exact _).
-     #[export] Instance qisok_iff : quotation_of M.Raw.isok_iff := ltac:(unfold_quotation_of (); exact _).
-     #[export] Instance qisok_Ok : quotation_of M.Raw.isok_Ok := ltac:(unfold_quotation_of (); exact _).
-     #[export] Instance qIn_1 : quotation_of M.Raw.In_1 := ltac:(unfold_quotation_of (); exact _).
-     #[export] Instance qIn_compat : quotation_of M.Raw.In_compat := ltac:(unfold_quotation_of (); exact _).
-     #[export] Instance qIn_node_iff : quotation_of M.Raw.In_node_iff := ltac:(unfold_quotation_of (); exact _).
-     #[export] Instance qIn_leaf_iff : quotation_of M.Raw.In_leaf_iff := ltac:(unfold_quotation_of (); exact _).*)
-     #[export] Instance qlt_leaf : quotation_of M.Raw.lt_leaf := ltac:(unfold_quotation_of (); exact _).
-     #[export] Instance qgt_leaf : quotation_of M.Raw.gt_leaf := ltac:(unfold_quotation_of (); exact _).
-     #[export] Instance qlt_tree_node : quotation_of M.Raw.lt_tree_node := ltac:(unfold_quotation_of (); exact _).
-     #[export] Instance qgt_tree_node : quotation_of M.Raw.gt_tree_node := ltac:(unfold_quotation_of (); exact _).
-     #[export] Instance qlt_tree_not_in : quotation_of M.Raw.lt_tree_not_in := ltac:(unfold_quotation_of (); exact _).
-     #[export] Instance qlt_tree_trans : quotation_of M.Raw.lt_tree_trans := ltac:(unfold_quotation_of (); exact _).
-     #[export] Instance qgt_tree_not_in : quotation_of M.Raw.gt_tree_not_in := ltac:(unfold_quotation_of (); exact _).
-     #[export] Instance qgt_tree_trans : quotation_of M.Raw.gt_tree_trans := ltac:(unfold_quotation_of (); exact _).
-     #[export] Instance qlt_tree_compat : quotation_of M.Raw.lt_tree_compat := ltac:(unfold_quotation_of (); exact _).
-     #[export] Instance qgt_tree_compat : quotation_of M.Raw.gt_tree_compat := ltac:(unfold_quotation_of (); exact _).
-     #[export] Instance qempty_spec : quotation_of M.Raw.empty_spec := ltac:(unfold_quotation_of (); exact _).
-     #[export] Instance qempty_ok : quotation_of M.Raw.empty_ok := ltac:(unfold_quotation_of (); exact _).
-     (*#[export] Instance qis_empty_spec : quotation_of M.Raw.is_empty_spec := ltac:(unfold_quotation_of (); exact _).
-     #[export] Instance qmem_spec : quotation_of M.Raw.mem_spec := ltac:(unfold_quotation_of (); exact _).
-     #[export] Instance qmin_elt_equation : quotation_of M.Raw.min_elt_equation := ltac:(unfold_quotation_of (); exact _).
-     #[export] Instance qmax_elt_equation : quotation_of M.Raw.max_elt_equation := ltac:(unfold_quotation_of (); exact _).
-     #[export] Instance qmin_elt_spec1 : quotation_of M.Raw.min_elt_spec1 := ltac:(unfold_quotation_of (); exact _).
-     #[export] Instance qmin_elt_spec2 : quotation_of M.Raw.min_elt_spec2 := ltac:(unfold_quotation_of (); exact _).
-     #[export] Instance qmin_elt_spec3 : quotation_of M.Raw.min_elt_spec3 := ltac:(unfold_quotation_of (); exact _).
-     #[export] Instance qmax_elt_spec1 : quotation_of M.Raw.max_elt_spec1 := ltac:(unfold_quotation_of (); exact _).
-     #[export] Instance qmax_elt_spec2 : quotation_of M.Raw.max_elt_spec2 := ltac:(unfold_quotation_of (); exact _).
-     #[export] Instance qmax_elt_spec3 : quotation_of M.Raw.max_elt_spec3 := ltac:(unfold_quotation_of (); exact _).
-     #[export] Instance qchoose_spec1 : quotation_of M.Raw.choose_spec1 := ltac:(unfold_quotation_of (); exact _).
-     #[export] Instance qchoose_spec2 : quotation_of M.Raw.choose_spec2 := ltac:(unfold_quotation_of (); exact _).
-     #[export] Instance qchoose_spec3 : quotation_of M.Raw.choose_spec3 := ltac:(unfold_quotation_of (); exact _).
-     #[export] Instance qelements_spec1' : quotation_of M.Raw.elements_spec1' := ltac:(unfold_quotation_of (); exact _).
-     #[export] Instance qelements_spec1 : quotation_of M.Raw.elements_spec1 := ltac:(unfold_quotation_of (); exact _).
-     #[export] Instance qelements_spec2' : quotation_of M.Raw.elements_spec2' := ltac:(unfold_quotation_of (); exact _).
-     #[export] Instance qelements_spec2 : quotation_of M.Raw.elements_spec2 := ltac:(unfold_quotation_of (); exact _).
-     #[export] Instance qelements_spec2w : quotation_of M.Raw.elements_spec2w := ltac:(unfold_quotation_of (); exact _).
-     #[export] Instance qelements_aux_cardinal : quotation_of M.Raw.elements_aux_cardinal := ltac:(unfold_quotation_of (); exact _).
-     #[export] Instance qelements_cardinal : quotation_of M.Raw.elements_cardinal := ltac:(unfold_quotation_of (); exact _).
-     #[export] Instance qcardinal_spec : quotation_of M.Raw.cardinal_spec := ltac:(unfold_quotation_of (); exact _).
-     #[export] Instance qelements_app : quotation_of M.Raw.elements_app := ltac:(unfold_quotation_of (); exact _).
-     #[export] Instance qelements_node : quotation_of M.Raw.elements_node := ltac:(unfold_quotation_of (); exact _).
-     #[export] Instance qrev_elements_app : quotation_of M.Raw.rev_elements_app := ltac:(unfold_quotation_of (); exact _).
-     #[export] Instance qrev_elements_node : quotation_of M.Raw.rev_elements_node := ltac:(unfold_quotation_of (); exact _).
-     #[export] Instance qrev_elements_rev : quotation_of M.Raw.rev_elements_rev := ltac:(unfold_quotation_of (); exact _).
-     #[export] Instance qsorted_app_inv : quotation_of M.Raw.sorted_app_inv := ltac:(unfold_quotation_of (); exact _).
-     #[export] Instance qelements_sort_ok : quotation_of M.Raw.elements_sort_ok := ltac:(unfold_quotation_of (); exact _).
-     #[export] Instance qfor_all_spec : quotation_of M.Raw.for_all_spec := ltac:(unfold_quotation_of (); exact _).
-     #[export] Instance qexists_spec : quotation_of M.Raw.exists_spec := ltac:(unfold_quotation_of (); exact _).
-     #[export] Instance qfold_spec' : quotation_of M.Raw.fold_spec' := ltac:(unfold_quotation_of (); exact _).
-     #[export] Instance qfold_spec : quotation_of M.Raw.fold_spec := ltac:(unfold_quotation_of (); exact _).
-     #[export] Instance qsubsetl_spec : quotation_of M.Raw.subsetl_spec := ltac:(unfold_quotation_of (); exact _).
-     #[export] Instance qsubsetr_spec : quotation_of M.Raw.subsetr_spec := ltac:(unfold_quotation_of (); exact _).
-     #[export] Instance qsubset_spec : quotation_of M.Raw.subset_spec := ltac:(unfold_quotation_of (); exact _).
-     #[export] Instance qeq : quotation_of M.Raw.eq := ltac:(unfold_quotation_of (); exact _).
-     #[export] Instance qeq_equiv : quotation_of M.Raw.eq_equiv := ltac:(unfold_quotation_of (); exact _).
-     #[export] Instance qeq_Leq : quotation_of M.Raw.eq_Leq := ltac:(unfold_quotation_of (); exact _).
-     #[export] Instance qlt : quotation_of M.Raw.lt := ltac:(unfold_quotation_of (); exact _).
-     #[export] Instance qlt_strorder : quotation_of M.Raw.lt_strorder := ltac:(unfold_quotation_of (); exact _).
-     #[export] Instance qlt_compat : quotation_of M.Raw.lt_compat := ltac:(unfold_quotation_of (); exact _).
-     #[export] Instance qflatten_e : quotation_of M.Raw.flatten_e := ltac:(unfold_quotation_of (); exact _).
-     #[export] Instance qflatten_e_elements : quotation_of M.Raw.flatten_e_elements := ltac:(unfold_quotation_of (); exact _).
-     #[export] Instance qcons_1 : quotation_of M.Raw.cons_1 := ltac:(unfold_quotation_of (); exact _).
-     #[export] Instance qCmp : quotation_of M.Raw.Cmp := ltac:(unfold_quotation_of (); exact _).
-     #[export] Instance qcompare_end_Cmp : quotation_of M.Raw.compare_end_Cmp := ltac:(unfold_quotation_of (); exact _).
-     #[export] Instance qcompare_more_Cmp : quotation_of M.Raw.compare_more_Cmp := ltac:(unfold_quotation_of (); exact _).
-     #[export] Instance qcompare_cont_Cmp : quotation_of M.Raw.compare_cont_Cmp := ltac:(unfold_quotation_of (); exact _).
-     #[export] Instance qcompare_Cmp : quotation_of M.Raw.compare_Cmp := ltac:(unfold_quotation_of (); exact _).
-     #[export] Instance qcompare_spec : quotation_of M.Raw.compare_spec := ltac:(unfold_quotation_of (); exact _).
-     #[export] Instance qequal_spec : quotation_of M.Raw.equal_spec := ltac:(unfold_quotation_of (); exact _).
-     #[export] Instance qmindepth_maxdepth : quotation_of M.Raw.mindepth_maxdepth := ltac:(unfold_quotation_of (); exact _).
-     #[export] Instance qmaxdepth_cardinal : quotation_of M.Raw.maxdepth_cardinal := ltac:(unfold_quotation_of (); exact _).
-     #[export] Instance qmindepth_cardinal : quotation_of M.Raw.mindepth_cardinal := ltac:(unfold_quotation_of (); exact _).
-     #[export] Instance qmaxdepth_log_cardinal : quotation_of M.Raw.maxdepth_log_cardinal := ltac:(unfold_quotation_of (); exact _).
-     #[export] Instance qmindepth_log_cardinal : quotation_of M.Raw.mindepth_log_cardinal := ltac:(unfold_quotation_of (); exact _).
-     #[export] Instance qremove_min_equation : quotation_of M.Raw.remove_min_equation := ltac:(unfold_quotation_of (); exact _).
-     #[export] Instance qinter_equation : quotation_of M.Raw.inter_equation := ltac:(unfold_quotation_of (); exact _).
-     #[export] Instance qdiff_equation : quotation_of M.Raw.diff_equation := ltac:(unfold_quotation_of (); exact _).
-     #[export] Instance qunion_equation : quotation_of M.Raw.union_equation := ltac:(unfold_quotation_of (); exact _).*)
-     #[export] Instance qsingleton_spec : quotation_of M.Raw.singleton_spec := ltac:(unfold_quotation_of (); exact _).
-     #[export] Instance qsingleton_ok : quotation_of M.Raw.singleton_ok := ltac:(unfold_quotation_of (); exact _).
-     #[export] Instance qcreate_spec : quotation_of M.Raw.create_spec := ltac:(unfold_quotation_of (); exact _).
-     #[export] Instance qcreate_ok : quotation_of M.Raw.create_ok := ltac:(unfold_quotation_of (); exact _).
-     #[export] Instance qbal_spec : quotation_of M.Raw.bal_spec := ltac:(unfold_quotation_of (); exact _).
-     #[export] Instance qbal_ok : quotation_of M.Raw.bal_ok := ltac:(unfold_quotation_of (); exact _).
-     #[export] Instance qadd_spec' : quotation_of M.Raw.add_spec' := ltac:(unfold_quotation_of (); exact _).
-     #[export] Instance qadd_spec : quotation_of M.Raw.add_spec := ltac:(unfold_quotation_of (); exact _).
-     Instance: debug_opt := true.
-     Fail #[export] Instance qadd_ok : quotation_of M.Raw.add_ok := ltac:(unfold_quotation_of (); exact _).
-     #[export] Instance qjoin_spec : quotation_of M.Raw.join_spec := ltac:(unfold_quotation_of (); exact _).
-     #[export] Instance qjoin_ok : quotation_of M.Raw.join_ok := ltac:(unfold_quotation_of (); exact _).
-     #[export] Instance qremove_min_spec : quotation_of M.Raw.remove_min_spec := ltac:(unfold_quotation_of (); exact _).
-     #[export] Instance qremove_min_ok : quotation_of M.Raw.remove_min_ok := ltac:(unfold_quotation_of (); exact _).
-     #[export] Instance qremove_min_gt_tree : quotation_of M.Raw.remove_min_gt_tree := ltac:(unfold_quotation_of (); exact _).
-     #[export] Instance qmerge_spec : quotation_of M.Raw.merge_spec := ltac:(unfold_quotation_of (); exact _).
-     #[export] Instance qmerge_ok : quotation_of M.Raw.merge_ok := ltac:(unfold_quotation_of (); exact _).
-     #[export] Instance qremove_spec : quotation_of M.Raw.remove_spec := ltac:(unfold_quotation_of (); exact _).
-     #[export] Instance qremove_ok : quotation_of M.Raw.remove_ok := ltac:(unfold_quotation_of (); exact _).
-     #[export] Instance qconcat_spec : quotation_of M.Raw.concat_spec := ltac:(unfold_quotation_of (); exact _).
-     #[export] Instance qconcat_ok : quotation_of M.Raw.concat_ok := ltac:(unfold_quotation_of (); exact _).
-     #[export] Instance qsplit_spec1 : quotation_of M.Raw.split_spec1 := ltac:(unfold_quotation_of (); exact _).
-     #[export] Instance qsplit_spec2 : quotation_of M.Raw.split_spec2 := ltac:(unfold_quotation_of (); exact _).
-     #[export] Instance qsplit_spec3 : quotation_of M.Raw.split_spec3 := ltac:(unfold_quotation_of (); exact _).
-     #[export] Instance qsplit_ok : quotation_of M.Raw.split_ok := ltac:(unfold_quotation_of (); exact _).
-     #[export] Instance qsplit_ok1 : quotation_of M.Raw.split_ok1 := ltac:(unfold_quotation_of (); exact _).
-     #[export] Instance qsplit_ok2 : quotation_of M.Raw.split_ok2 := ltac:(unfold_quotation_of (); exact _).
-     #[export] Instance qinter_spec_ok : quotation_of M.Raw.inter_spec_ok := ltac:(unfold_quotation_of (); exact _).
-     #[export] Instance qinter_spec : quotation_of M.Raw.inter_spec := ltac:(unfold_quotation_of (); exact _).
-     #[export] Instance qinter_ok : quotation_of M.Raw.inter_ok := ltac:(unfold_quotation_of (); exact _).
-     #[export] Instance qdiff_spec_ok : quotation_of M.Raw.diff_spec_ok := ltac:(unfold_quotation_of (); exact _).
-     #[export] Instance qdiff_spec : quotation_of M.Raw.diff_spec := ltac:(unfold_quotation_of (); exact _).
-     #[export] Instance qdiff_ok : quotation_of M.Raw.diff_ok := ltac:(unfold_quotation_of (); exact _).
-     #[export] Instance qunion_spec : quotation_of M.Raw.union_spec := ltac:(unfold_quotation_of (); exact _).
-     #[export] Instance qunion_ok : quotation_of M.Raw.union_ok := ltac:(unfold_quotation_of (); exact _).
-     #[export] Instance qfilter_spec : quotation_of M.Raw.filter_spec := ltac:(unfold_quotation_of (); exact _).
-     #[export] Instance qfilter_weak_spec : quotation_of M.Raw.filter_weak_spec := ltac:(unfold_quotation_of (); exact _).
-     #[export] Instance qfilter_ok : quotation_of M.Raw.filter_ok := ltac:(unfold_quotation_of (); exact _).
-     #[export] Instance qpartition_spec1' : quotation_of M.Raw.partition_spec1' := ltac:(unfold_quotation_of (); exact _).
-     #[export] Instance qpartition_spec2' : quotation_of M.Raw.partition_spec2' := ltac:(unfold_quotation_of (); exact _).
-     #[export] Instance qpartition_spec1 : quotation_of M.Raw.partition_spec1 := ltac:(unfold_quotation_of (); exact _).
-     #[export] Instance qpartition_spec2 : quotation_of M.Raw.partition_spec2 := ltac:(unfold_quotation_of (); exact _).
-     #[export] Instance qpartition_ok1 : quotation_of M.Raw.partition_ok1 := ltac:(unfold_quotation_of (); exact _).
-     #[export] Instance qpartition_ok2 : quotation_of M.Raw.partition_ok2 := ltac:(unfold_quotation_of (); exact _).
-      *)
-    End Raw.
-    Export (hints) Raw.
-    #[export] Instance qt : quotation_of M.t := ltac:(unfold_quotation_of (); exact _).
-    #[export] Instance qempty : quotation_of M.empty := ltac:(unfold_quotation_of (); exact _).
-    #[export] Instance qthis : quotation_of M.this := ltac:(unfold_quotation_of (); exact _).
-    #[export] Instance qis_empty : quotation_of M.is_empty := ltac:(unfold_quotation_of (); exact _).
-    #[export] Instance qmem : quotation_of M.mem := ltac:(unfold_quotation_of (); exact _).
-    #[export] Instance qadd : quotation_of M.add := ltac:(unfold_quotation_of (); exact _).
-    #[export] Instance qsingleton : quotation_of M.singleton := ltac:(unfold_quotation_of (); exact _).
-    #[export] Instance qremove : quotation_of M.remove := ltac:(unfold_quotation_of (); exact _).
-    #[export] Instance qunion : quotation_of M.union := ltac:(unfold_quotation_of (); exact _).
-    #[export] Instance qinter : quotation_of M.inter := ltac:(unfold_quotation_of (); exact _).
-    #[export] Instance qdiff : quotation_of M.diff := ltac:(unfold_quotation_of (); exact _).
-    #[export] Instance qequal : quotation_of M.equal := ltac:(unfold_quotation_of (); exact _).
-    #[export] Instance qsubset : quotation_of M.subset := ltac:(unfold_quotation_of (); exact _).
-    #[export] Instance qfold : quotation_of M.fold := ltac:(unfold_quotation_of (); exact _).
-    #[export] Instance qfor_all : quotation_of M.for_all := ltac:(unfold_quotation_of (); exact _).
-    #[export] Instance qexists_ : quotation_of M.exists_ := ltac:(unfold_quotation_of (); exact _).
-    #[export] Instance qfilter : quotation_of M.filter := ltac:(unfold_quotation_of (); exact _).
-    #[export] Instance qpartition : quotation_of M.partition := ltac:(unfold_quotation_of (); exact _).
-    #[export] Instance qcardinal : quotation_of M.cardinal := ltac:(unfold_quotation_of (); exact _).
-    #[export] Instance qelements : quotation_of M.elements := ltac:(unfold_quotation_of (); exact _).
-    #[export] Instance qchoose : quotation_of M.choose := ltac:(unfold_quotation_of (); exact _).
-    #[export] Instance qIn : quotation_of M.In := ltac:(unfold_quotation_of (); exact _).
-    #[export] Instance qIn_compat : quotation_of M.In_compat := ltac:(unfold_quotation_of (); exact _).
-    #[export] Instance qeq_equiv : quotation_of M.eq_equiv := ltac:(unfold_quotation_of (); exact _).
-    #[export] Instance qeq_dec : quotation_of M.eq_dec := ltac:(unfold_quotation_of (); exact _).
-    #[export] Instance qmem_spec : quotation_of M.mem_spec := ltac:(unfold_quotation_of (); exact _).
-    #[export] Instance qequal_spec : quotation_of M.equal_spec := ltac:(unfold_quotation_of (); exact _).
-    #[export] Instance qsubset_spec : quotation_of M.subset_spec := ltac:(unfold_quotation_of (); exact _).
-    #[export] Instance qempty_spec : quotation_of M.empty_spec := ltac:(unfold_quotation_of (); exact _).
-    #[export] Instance qis_empty_spec : quotation_of M.is_empty_spec := ltac:(unfold_quotation_of (); exact _).
-    #[export] Instance qadd_spec : quotation_of M.add_spec := ltac:(unfold_quotation_of (); exact _).
-    #[export] Instance qremove_spec : quotation_of M.remove_spec := ltac:(unfold_quotation_of (); exact _).
-    #[export] Instance qsingleton_spec : quotation_of M.singleton_spec := ltac:(unfold_quotation_of (); exact _).
-    #[export] Instance qunion_spec : quotation_of M.union_spec := ltac:(unfold_quotation_of (); exact _).
-    #[export] Instance qinter_spec : quotation_of M.inter_spec := ltac:(unfold_quotation_of (); exact _).
-    #[export] Instance qdiff_spec : quotation_of M.diff_spec := ltac:(unfold_quotation_of (); exact _).
-    #[export] Instance qfold_spec : quotation_of M.fold_spec := ltac:(unfold_quotation_of (); exact _).
-    #[export] Instance qcardinal_spec : quotation_of M.cardinal_spec := ltac:(unfold_quotation_of (); exact _).
-    #[export] Instance qfilter_spec : quotation_of M.filter_spec := ltac:(unfold_quotation_of (); exact _).
-    #[export] Instance qfor_all_spec : quotation_of M.for_all_spec := ltac:(unfold_quotation_of (); exact _).
-    #[export] Instance qexists_spec : quotation_of M.exists_spec := ltac:(unfold_quotation_of (); exact _).
-    #[export] Instance qpartition_spec1 : quotation_of M.partition_spec1 := ltac:(unfold_quotation_of (); exact _).
-    #[export] Instance qpartition_spec2 : quotation_of M.partition_spec2 := ltac:(unfold_quotation_of (); exact _).
-    #[export] Instance qelements_spec1 : quotation_of M.elements_spec1 := ltac:(unfold_quotation_of (); exact _).
-    #[export] Instance qelements_spec2w : quotation_of M.elements_spec2w := ltac:(unfold_quotation_of (); exact _).
-    #[export] Instance qchoose_spec1 : quotation_of M.choose_spec1 := ltac:(unfold_quotation_of (); exact _).
-    #[export] Instance qchoose_spec2 : quotation_of M.choose_spec2 := ltac:(unfold_quotation_of (); exact _).
-    #[export] Instance qcompare : quotation_of M.compare := ltac:(unfold_quotation_of (); exact _).
-    #[export] Instance qmin_elt : quotation_of M.min_elt := ltac:(unfold_quotation_of (); exact _).
-    #[export] Instance qmax_elt : quotation_of M.max_elt := ltac:(unfold_quotation_of (); exact _).
-    #[export] Instance qlt : quotation_of M.lt := ltac:(unfold_quotation_of (); exact _).
-    #[export] Instance qlt_strorder : quotation_of M.lt_strorder := ltac:(unfold_quotation_of (); exact _).
-    #[export] Instance qlt_compat : quotation_of M.lt_compat := ltac:(unfold_quotation_of (); exact _).
-    #[export] Instance qcompare_spec : quotation_of M.compare_spec := ltac:(unfold_quotation_of (); exact _).
-    #[export] Instance qelements_spec2 : quotation_of M.elements_spec2 := ltac:(unfold_quotation_of (); exact _).
-    #[export] Instance qmin_elt_spec1 : quotation_of M.min_elt_spec1 := ltac:(unfold_quotation_of (); exact _).
-    #[export] Instance qmin_elt_spec2 : quotation_of M.min_elt_spec2 := ltac:(unfold_quotation_of (); exact _).
-    #[export] Instance qmin_elt_spec3 : quotation_of M.min_elt_spec3 := ltac:(unfold_quotation_of (); exact _).
-    #[export] Instance qmax_elt_spec1 : quotation_of M.max_elt_spec1 := ltac:(unfold_quotation_of (); exact _).
-    #[export] Instance qmax_elt_spec2 : quotation_of M.max_elt_spec2 := ltac:(unfold_quotation_of (); exact _).
-    #[export] Instance qmax_elt_spec3 : quotation_of M.max_elt_spec3 := ltac:(unfold_quotation_of (); exact _).
-    #[export] Instance qchoose_spec3 : quotation_of M.choose_spec3 := ltac:(unfold_quotation_of (); exact _).
+  Module MSetList.
+    Module Type MakeSig (T : OrderedType) := Nop <+ MSetList.Make T.
+    Module Type QuotationOfMake (T : OrderedType) (M : MakeSig T).
+      Module qRaw.
+        (*Module qMX := QuotationOfOrderedTypeFacts T M.Raw.MX qT.*)
+        (*Module qML := QuotationOfOrderedTypeLists T M.Raw.ML qT.*)
+        #[export] Declare Instance qelt : quotation_of M.Raw.elt.
+        #[export] Declare Instance qt : quotation_of M.Raw.t.
+        #[export] Declare Instance qempty : quotation_of M.Raw.empty.
+        #[export] Declare Instance qis_empty : quotation_of M.Raw.is_empty.
+        #[export] Declare Instance qmem : quotation_of M.Raw.mem.
+        #[export] Declare Instance qadd : quotation_of M.Raw.add.
+        #[export] Declare Instance qsingleton : quotation_of M.Raw.singleton.
+        #[export] Declare Instance qremove : quotation_of M.Raw.remove.
+        #[export] Declare Instance qunion : quotation_of M.Raw.union.
+        #[export] Declare Instance qinter : quotation_of M.Raw.inter.
+        #[export] Declare Instance qdiff : quotation_of M.Raw.diff.
+        #[export] Declare Instance qequal : quotation_of M.Raw.equal.
+        #[export] Declare Instance qsubset : quotation_of M.Raw.subset.
+        #[export] Declare Instance qfold : quotation_of M.Raw.fold.
+        #[export] Declare Instance qfilter : quotation_of M.Raw.filter.
+        #[export] Declare Instance qfor_all : quotation_of M.Raw.for_all.
+        #[export] Declare Instance qexists_ : quotation_of M.Raw.exists_.
+        #[export] Declare Instance qpartition : quotation_of M.Raw.partition.
+        #[export] Declare Instance qcardinal : quotation_of M.Raw.cardinal.
+        #[export] Declare Instance qelements : quotation_of M.Raw.elements.
+        #[export] Declare Instance qmin_elt : quotation_of M.Raw.min_elt.
+        #[export] Declare Instance qmax_elt : quotation_of M.Raw.max_elt.
+        #[export] Declare Instance qchoose : quotation_of M.Raw.choose.
+        #[export] Declare Instance qcompare : quotation_of M.Raw.compare.
+        #[export] Declare Instance qinf : quotation_of M.Raw.inf.
+        #[export] Declare Instance qisok : quotation_of M.Raw.isok.
+        #[export] Declare Instance qIsOk : quotation_of M.Raw.IsOk.
+        #[export] Declare Instance qOk : quotation_of M.Raw.Ok.
+        #[export] Declare Instance qok : quotation_of (@M.Raw.ok).
+        #[export] Declare Instance qSort_Ok : quotation_of M.Raw.Sort_Ok.
+        #[export] Declare Instance qinf_iff : quotation_of M.Raw.inf_iff.
+        #[export] Declare Instance qisok_iff : quotation_of M.Raw.isok_iff.
+        #[export] Declare Instance qisok_Ok : quotation_of M.Raw.isok_Ok.
+        #[export] Declare Instance qEqual : quotation_of M.Raw.Equal.
+        #[export] Declare Instance qSubset : quotation_of M.Raw.Subset.
+        #[export] Declare Instance qEmpty : quotation_of M.Raw.Empty.
+        #[export] Declare Instance qFor_all : quotation_of M.Raw.For_all.
+        #[export] Declare Instance qExists : quotation_of M.Raw.Exists.
+        #[export] Declare Instance qmem_spec : quotation_of M.Raw.mem_spec.
+        #[export] Declare Instance qadd_inf : quotation_of M.Raw.add_inf.
+        #[export] Declare Instance qadd_ok : quotation_of M.Raw.add_ok.
+        #[export] Declare Instance qadd_spec : quotation_of M.Raw.add_spec.
+        #[export] Declare Instance qremove_inf : quotation_of M.Raw.remove_inf.
+        #[export] Declare Instance qremove_ok : quotation_of M.Raw.remove_ok.
+        #[export] Declare Instance qremove_spec : quotation_of M.Raw.remove_spec.
+        #[export] Declare Instance qsingleton_ok : quotation_of M.Raw.singleton_ok.
+        #[export] Declare Instance qsingleton_spec : quotation_of M.Raw.singleton_spec.
+        #[export] Declare Instance qunion_inf : quotation_of M.Raw.union_inf.
+        #[export] Declare Instance qunion_ok : quotation_of M.Raw.union_ok.
+        #[export] Declare Instance qunion_spec : quotation_of M.Raw.union_spec.
+        #[export] Declare Instance qinter_inf : quotation_of M.Raw.inter_inf.
+        #[export] Declare Instance qinter_ok : quotation_of M.Raw.inter_ok.
+        #[export] Declare Instance qinter_spec : quotation_of M.Raw.inter_spec.
+        #[export] Declare Instance qdiff_inf : quotation_of M.Raw.diff_inf.
+        #[export] Declare Instance qdiff_ok : quotation_of M.Raw.diff_ok.
+        #[export] Declare Instance qdiff_spec : quotation_of M.Raw.diff_spec.
+        #[export] Declare Instance qequal_spec : quotation_of M.Raw.equal_spec.
+        #[export] Declare Instance qsubset_spec : quotation_of M.Raw.subset_spec.
+        #[export] Declare Instance qempty_ok : quotation_of M.Raw.empty_ok.
+        #[export] Declare Instance qempty_spec : quotation_of M.Raw.empty_spec.
+        #[export] Declare Instance qis_empty_spec : quotation_of M.Raw.is_empty_spec.
+        #[export] Declare Instance qelements_spec1 : quotation_of M.Raw.elements_spec1.
+        #[export] Declare Instance qelements_spec2 : quotation_of M.Raw.elements_spec2.
+        #[export] Declare Instance qelements_spec2w : quotation_of M.Raw.elements_spec2w.
+        #[export] Declare Instance qmin_elt_spec1 : quotation_of M.Raw.min_elt_spec1.
+        #[export] Declare Instance qmin_elt_spec2 : quotation_of M.Raw.min_elt_spec2.
+        #[export] Declare Instance qmin_elt_spec3 : quotation_of M.Raw.min_elt_spec3.
+        #[export] Declare Instance qmax_elt_spec1 : quotation_of M.Raw.max_elt_spec1.
+        #[export] Declare Instance qmax_elt_spec2 : quotation_of M.Raw.max_elt_spec2.
+        #[export] Declare Instance qmax_elt_spec3 : quotation_of M.Raw.max_elt_spec3.
+        #[export] Declare Instance qchoose_spec1 : quotation_of M.Raw.choose_spec1.
+        #[export] Declare Instance qchoose_spec2 : quotation_of M.Raw.choose_spec2.
+        #[export] Declare Instance qchoose_spec3 : quotation_of M.Raw.choose_spec3.
+        #[export] Declare Instance qfold_spec : quotation_of M.Raw.fold_spec.
+        #[export] Declare Instance qcardinal_spec : quotation_of M.Raw.cardinal_spec.
+        #[export] Declare Instance qfilter_inf : quotation_of M.Raw.filter_inf.
+        #[export] Declare Instance qfilter_ok : quotation_of M.Raw.filter_ok.
+        #[export] Declare Instance qfilter_spec : quotation_of M.Raw.filter_spec.
+        #[export] Declare Instance qfor_all_spec : quotation_of M.Raw.for_all_spec.
+        #[export] Declare Instance qexists_spec : quotation_of M.Raw.exists_spec.
+        #[export] Declare Instance qpartition_inf1 : quotation_of M.Raw.partition_inf1.
+        #[export] Declare Instance qpartition_inf2 : quotation_of M.Raw.partition_inf2.
+        #[export] Declare Instance qpartition_ok1 : quotation_of M.Raw.partition_ok1.
+        #[export] Declare Instance qpartition_ok2 : quotation_of M.Raw.partition_ok2.
+        #[export] Declare Instance qpartition_spec1 : quotation_of M.Raw.partition_spec1.
+        #[export] Declare Instance qpartition_spec2 : quotation_of M.Raw.partition_spec2.
+        #[export] Declare Instance qIn : quotation_of M.Raw.In.
+        #[export] Declare Instance qIn_compat : quotation_of M.Raw.In_compat.
+        #[export] Declare Instance qeq : quotation_of M.Raw.eq.
+        #[export] Declare Instance qeq_equiv : quotation_of M.Raw.eq_equiv.
+        #[export] Declare Instance qlt : quotation_of M.Raw.lt.
+        #[export] Declare Instance qlt_strorder : quotation_of M.Raw.lt_strorder.
+        #[export] Declare Instance qlt_compat : quotation_of M.Raw.lt_compat.
+        #[export] Declare Instance qcompare_spec_aux : quotation_of M.Raw.compare_spec_aux.
+        #[export] Declare Instance qcompare_spec : quotation_of M.Raw.compare_spec.
+      End qRaw.
+      #[export] Declare Instance qelt : quotation_of M.elt.
+      #[export] Declare Instance qt_ : inductive_quotation_of M.t_.
+      #[export] Declare Instance qthis : quotation_of M.this.
+      #[export] Declare Instance qis_ok : quotation_of M.is_ok.
+      #[export] Declare Instance qt : quotation_of M.t.
+      #[export] Declare Instance qIn : quotation_of M.In.
+      #[export] Declare Instance qEqual : quotation_of M.Equal.
+      #[export] Declare Instance qSubset : quotation_of M.Subset.
+      #[export] Declare Instance qEmpty : quotation_of M.Empty.
+      #[export] Declare Instance qFor_all : quotation_of M.For_all.
+      #[export] Declare Instance qExists : quotation_of M.Exists.
+      #[export] Declare Instance qmem : quotation_of M.mem.
+      #[export] Declare Instance qadd : quotation_of M.add.
+      #[export] Declare Instance qremove : quotation_of M.remove.
+      #[export] Declare Instance qsingleton : quotation_of M.singleton.
+      #[export] Declare Instance qunion : quotation_of M.union.
+      #[export] Declare Instance qinter : quotation_of M.inter.
+      #[export] Declare Instance qdiff : quotation_of M.diff.
+      #[export] Declare Instance qequal : quotation_of M.equal.
+      #[export] Declare Instance qsubset : quotation_of M.subset.
+      #[export] Declare Instance qempty : quotation_of M.empty.
+      #[export] Declare Instance qis_empty : quotation_of M.is_empty.
+      #[export] Declare Instance qelements : quotation_of M.elements.
+      #[export] Declare Instance qchoose : quotation_of M.choose.
+      #[export] Declare Instance qfold : quotation_of M.fold.
+      #[export] Declare Instance qcardinal : quotation_of M.cardinal.
+      #[export] Declare Instance qfilter : quotation_of M.filter.
+      #[export] Declare Instance qfor_all : quotation_of M.for_all.
+      #[export] Declare Instance qexists_ : quotation_of M.exists_.
+      #[export] Declare Instance qpartition : quotation_of M.partition.
+      #[export] Declare Instance qIn_compat : quotation_of M.In_compat.
+      #[export] Declare Instance qeq : quotation_of M.eq.
+      #[export] Declare Instance qeq_equiv : quotation_of M.eq_equiv.
+      #[export] Declare Instance qeq_dec : quotation_of M.eq_dec.
+      #[export] Declare Instance qmem_spec : quotation_of M.mem_spec.
+      #[export] Declare Instance qequal_spec : quotation_of M.equal_spec.
+      #[export] Declare Instance qsubset_spec : quotation_of M.subset_spec.
+      #[export] Declare Instance qempty_spec : quotation_of M.empty_spec.
+      #[export] Declare Instance qis_empty_spec : quotation_of M.is_empty_spec.
+      #[export] Declare Instance qadd_spec : quotation_of M.add_spec.
+      #[export] Declare Instance qremove_spec : quotation_of M.remove_spec.
+      #[export] Declare Instance qsingleton_spec : quotation_of M.singleton_spec.
+      #[export] Declare Instance qunion_spec : quotation_of M.union_spec.
+      #[export] Declare Instance qinter_spec : quotation_of M.inter_spec.
+      #[export] Declare Instance qdiff_spec : quotation_of M.diff_spec.
+      #[export] Declare Instance qfold_spec : quotation_of M.fold_spec.
+      #[export] Declare Instance qcardinal_spec : quotation_of M.cardinal_spec.
+      #[export] Declare Instance qfilter_spec : quotation_of M.filter_spec.
+      #[export] Declare Instance qfor_all_spec : quotation_of M.for_all_spec.
+      #[export] Declare Instance qexists_spec : quotation_of M.exists_spec.
+      #[export] Declare Instance qpartition_spec1 : quotation_of M.partition_spec1.
+      #[export] Declare Instance qpartition_spec2 : quotation_of M.partition_spec2.
+      #[export] Declare Instance qelements_spec1 : quotation_of M.elements_spec1.
+      #[export] Declare Instance qelements_spec2w : quotation_of M.elements_spec2w.
+      #[export] Declare Instance qchoose_spec1 : quotation_of M.choose_spec1.
+      #[export] Declare Instance qchoose_spec2 : quotation_of M.choose_spec2.
+      #[export] Declare Instance qcompare : quotation_of M.compare.
+      #[export] Declare Instance qmin_elt : quotation_of M.min_elt.
+      #[export] Declare Instance qmax_elt : quotation_of M.max_elt.
+      #[export] Declare Instance qlt : quotation_of M.lt.
+      #[export] Declare Instance qlt_strorder : quotation_of M.lt_strorder.
+      #[export] Declare Instance qlt_compat : quotation_of M.lt_compat.
+      #[export] Declare Instance qcompare_spec : quotation_of M.compare_spec.
+      #[export] Declare Instance qelements_spec2 : quotation_of M.elements_spec2.
+      #[export] Declare Instance qmin_elt_spec1 : quotation_of M.min_elt_spec1.
+      #[export] Declare Instance qmin_elt_spec2 : quotation_of M.min_elt_spec2.
+      #[export] Declare Instance qmin_elt_spec3 : quotation_of M.min_elt_spec3.
+      #[export] Declare Instance qmax_elt_spec1 : quotation_of M.max_elt_spec1.
+      #[export] Declare Instance qmax_elt_spec2 : quotation_of M.max_elt_spec2.
+      #[export] Declare Instance qmax_elt_spec3 : quotation_of M.max_elt_spec3.
+      #[export] Declare Instance qchoose_spec3 : quotation_of M.choose_spec3.
+    End QuotationOfMake.
 
-  #[export] Declare Instance qcompare_spec : quotation_of W.compare_spec.
-  #[export] Declare Instance qelements_spec2 : quotation_of W.elements_spec2.
-  #[export] Declare Instance qmin_elt_spec1 : quotation_of W.min_elt_spec1.
-  #[export] Declare Instance qmin_elt_spec2 : quotation_of W.min_elt_spec2.
-  #[export] Declare Instance qmin_elt_spec3 : quotation_of W.min_elt_spec3.
-  #[export] Declare Instance qmax_elt_spec1 : quotation_of W.max_elt_spec1.
-  #[export] Declare Instance qmax_elt_spec2 : quotation_of W.max_elt_spec2.
-  #[export] Declare Instance qmax_elt_spec3 : quotation_of W.max_elt_spec3.
-  #[export] Declare Instance qchoose_spec3 : quotation_of W.choose_spec3.
+    Module Type MakeWithLeibnizSig (T : OrderedTypeWithLeibniz) := Nop <+ MSetList.MakeWithLeibniz T.
+    Module Type QuotationOfMakeWithLeibniz (T : OrderedTypeWithLeibniz) (M : MakeWithLeibnizSig T).
+      Include QuotationOfMake T M.
+      #[export] Declare Instance qeq_leibniz_list : quotation_of M.eq_leibniz_list.
+      #[export] Declare Instance qeq_leibniz : quotation_of M.eq_leibniz.
+    End QuotationOfMakeWithLeibniz.
+  End MSetList.
+End MSets.
 
-  End ExtraQuotationOfMake.
+Module QuoteMSetAVL (T : OrderedType) (M : MSetAVL.MakeSig T) (Import MOrdProperties : OrdPropertiesSig M) (Import qT : QuotationOfOrderedType T) (Import qM : MSetAVL.QuotationOfMake T M) (qMOrdProperties : QuotationOfOrdProperties M MOrdProperties qT).
+  Export (hints) qT qM qMOrdProperties.
+  Include QuoteSets M MOrdProperties qT qM qMOrdProperties.
 
-Print MSetAVL.Make.
-
-Module QuoteMSetAVL (T : OrderedType) (M : MSetAVL_MakeSig T) (Import qT : QuotationOfOrderedType T) (Import qM : QuotationOfSetsOn T M).
-  Module Import QM := QuoteSetsOn T M qT qM.
-  Export (hints) QM.
-
-  Module Definitions.
-    Include QM.OrdDefinitions.
-
+  Module Raw.
     Scheme Induction for M.Raw.tree Sort Type.
     Scheme Induction for M.Raw.tree Sort Set.
     Scheme Induction for M.Raw.tree Sort Prop.
@@ -814,18 +965,14 @@ Module QuoteMSetAVL (T : OrderedType) (M : MSetAVL_MakeSig T) (Import qT : Quota
     Scheme Minimality for M.Raw.tree Sort Prop.
 
     Section with_t.
-      Context {quote_T_t : ground_quotable T.t}
-              {qRaw_tree : inductive_quotation_of M.Raw.tree}
-              {qRaw_bst : inductive_quotation_of M.Raw.bst}
-              {qt_ : inductive_quotation_of M.t_}.
+      Context {quote_T_t : ground_quotable T.t}.
 
-      #[export] Instance quote_M_Raw_t : ground_quotable M.Raw.t := (ltac:(induction 1; exact _)).
-      Fixpoint M_Raw_lt_tree_dec x t : { M.Raw.lt_tree x t } + {~ M.Raw.lt_tree x t}.
+      Fixpoint lt_tree_dec x t : { M.Raw.lt_tree x t } + {~ M.Raw.lt_tree x t}.
       Proof.
         refine match t with
                | M.Raw.Leaf => left _
                | M.Raw.Node z l n r
-                 => match T.compare n x as c, M_Raw_lt_tree_dec x l, M_Raw_lt_tree_dec x r return CompareSpec _ _ _ c -> _ with
+                 => match T.compare n x as c, lt_tree_dec x l, lt_tree_dec x r return CompareSpec _ _ _ c -> _ with
                     | Lt, left p2, left p3 => fun pfc => left _
                     | _, right pf, _ => fun pfc => right _
                     | _, _, right pf => fun pfc => right _
@@ -841,12 +988,12 @@ Module QuoteMSetAVL (T : OrderedType) (M : MSetAVL_MakeSig T) (Import qT : Quota
                     | intro f; apply pf; hnf in *; intros; apply f; constructor; (assumption + reflexivity)
                     | intro f; inversion pfc; eapply M.Raw.MX.lt_irrefl; (idtac + etransitivity); (eassumption + (eapply f; constructor; (idtac + symmetry); (eassumption + reflexivity))) ].
       Defined.
-      Fixpoint M_Raw_gt_tree_dec x t : { M.Raw.gt_tree x t } + {~ M.Raw.gt_tree x t}.
+      Fixpoint gt_tree_dec x t : { M.Raw.gt_tree x t } + {~ M.Raw.gt_tree x t}.
       Proof.
         refine match t with
                | M.Raw.Leaf => left _
                | M.Raw.Node z l n r
-                 => match T.compare n x as c, M_Raw_gt_tree_dec x l, M_Raw_gt_tree_dec x r return CompareSpec _ _ _ c -> _ with
+                 => match T.compare n x as c, gt_tree_dec x l, gt_tree_dec x r return CompareSpec _ _ _ c -> _ with
                     | Gt, left p2, left p3 => fun pfc => left _
                     | _, right pf, _ => fun pfc => right _
                     | _, _, right pf => fun pfc => right _
@@ -862,12 +1009,12 @@ Module QuoteMSetAVL (T : OrderedType) (M : MSetAVL_MakeSig T) (Import qT : Quota
                     | intro f; apply pf; hnf in *; intros; apply f; constructor; (assumption + reflexivity)
                     | intro f; inversion pfc; eapply M.Raw.MX.lt_irrefl; (idtac + etransitivity); (eassumption + (eapply f; constructor; (idtac + symmetry); (eassumption + reflexivity))) ].
       Defined.
-      Fixpoint M_Raw_bst_dec t : { M.Raw.bst t } + {~ M.Raw.bst t}.
+      Fixpoint bst_dec t : { M.Raw.bst t } + {~ M.Raw.bst t}.
       Proof.
         refine match t with
                | M.Raw.Leaf => left _
                | M.Raw.Node z l n r
-                 => match M_Raw_bst_dec l, M_Raw_bst_dec r, M_Raw_lt_tree_dec n l, M_Raw_gt_tree_dec n r with
+                 => match bst_dec l, bst_dec r, lt_tree_dec n l, gt_tree_dec n r with
                     | right pf, _, _, _ => right _
                     | _, right pf, _, _ => right _
                     | _, _, right pf, _ => right _
@@ -878,177 +1025,86 @@ Module QuoteMSetAVL (T : OrderedType) (M : MSetAVL_MakeSig T) (Import qT : Quota
           try solve [ constructor; assumption
                     | inversion 1; subst; auto ].
       Defined.
-      #[export] Instance quote_Raw_bst t : ground_quotable (M.Raw.bst t)
-        := ground_quotable_of_dec (@M_Raw_bst_dec t).
-      #[export] Instance quote_Raw_Ok s : ground_quotable (M.Raw.Ok s) := (ltac:(cbv [M.Raw.Ok]; exact _)).
-      #[export] Instance quote_t : ground_quotable M.t := ltac:(induction 1; exact _).
+      (* very slow :-( *)
+      #[export] Instance qlt_tree_dec : quotation_of (@lt_tree_dec) := ltac:(unfold_quotation_of (); exact _).
+      #[export] Instance qgt_tree_dec : quotation_of (@gt_tree_dec) := ltac:(unfold_quotation_of (); exact _).
+      #[export] Instance qbst_dec : quotation_of (@bst_dec) := ltac:(unfold_quotation_of (); exact _).
+      #[export] Instance quote_tree : ground_quotable M.Raw.tree := (ltac:(induction 1; exact _)).
+      #[export] Instance quote_bst t : ground_quotable (M.Raw.bst t)
+        := ground_quotable_of_dec (@bst_dec t).
+      #[export] Instance quote_Ok s : ground_quotable (M.Raw.Ok s) := (ltac:(cbv [M.Raw.Ok]; exact _)).
     End with_t.
-  End Definitions.
-  Include Definitions.
-  Module Export Instances.
-    Export QM.OrdInstances.
     #[export] Existing Instances
-     quote_M_Raw_t
-     quote_Raw_bst
-     quote_Raw_Ok
-     quote_t
+      qlt_tree_dec
+      qgt_tree_dec
+      qbst_dec
+      quote_tree
+      quote_bst
+      quote_Ok
     .
-  End Instances.
+  End Raw.
+  Export (hints) Raw.
+
+  #[export] Instance quote_t {quote_T_t : ground_quotable T.t} : ground_quotable M.t := ltac:(induction 1; exact _).
 End QuoteMSetAVL.
 
-Module QuoteUsualWSetsOn (E : UsualDecidableType) (Import M : WSetsOn E).
-  Module Import QM := QuoteWSetsOn E M.
+Module QuoteUsualWSetsOn (E : UsualDecidableType) (Import M : WSetsOn E) (MProperties : WPropertiesOnSig E M) (qE : QuotationOfUsualDecidableType E) (qM : QuotationOfWSetsOn E M) (qMProperties : QuotationOfWPropertiesOn E M MProperties).
+  Include QuoteWSetsOn E M MProperties qE qM qMProperties.
 
-  Module Definitions.
-    Notation quote_In := QM.quote_In.
-    Notation quote_Equal := QM.quote_Equal.
-    Notation quote_Subset := QM.quote_Subset.
-    Notation quote_Empty := QM.quote_Empty.
-    Notation quote_Add := QM.quote_Add.
-    Notation quote_neg_In := QM.quote_neg_In.
-    Notation quote_neg_Equal := QM.quote_neg_Equal.
-    Notation quote_neg_Subset := QM.quote_neg_Subset.
-    Notation quote_neg_Empty := QM.quote_neg_Empty.
-    Notation quote_neg_Add := QM.quote_neg_Add.
-
-    Section with_quote.
-      Context {qelt : quotation_of elt} {qt : quotation_of t}
-              {qIn : quotation_of In}
-              {qeq_dec : quotation_of eq_dec}
-              {qsubset_spec : quotation_of subset_spec}
-              {qempty : quotation_of empty}
-              {qadd : quotation_of add} {qelements : quotation_of elements}.
-
-      #[export] Instance quote_For_all {P s} {quote_elt : ground_quotable elt} {quote_P : forall x, ground_quotable (P x:Prop)} {qP : quotation_of P} {qs : quotation_of s} : ground_quotable (For_all P s)
-        := QM.quote_For_all.
-      Definition quote_Exists_dec {P} (P_dec : forall x, {P x} + {~P x}) {s} {quote_elt : ground_quotable elt} {qP_dec : quotation_of P_dec} {quote_P : forall x, ground_quotable (P x:Prop)} {qP : quotation_of P} {qs : quotation_of s} : ground_quotable (Exists P s)
-        := QM.quote_Exists_dec P_dec.
-      #[export] Instance quote_forall2_In {P s} {qP : quotation_of P} {qs : quotation_of s} {quote_elt : ground_quotable elt} {quote_P : forall x y, ground_quotable (P x y:Prop)} : ground_quotable (forall v1 v2, In v1 s -> In v2 s -> P v1 v2) := _.
-    End with_quote.
-  End Definitions.
-
-  Include Definitions.
-
-  Module Export Instances.
-    #[export] Existing Instances
-     QM.quote_In
-     QM.quote_Equal
-     QM.quote_Subset
-     QM.quote_Empty
-     QM.quote_Add
-     QM.quote_neg_In
-     QM.quote_neg_Equal
-     QM.quote_neg_Subset
-     QM.quote_neg_Empty
-     QM.quote_neg_Add
-     quote_For_all
-     quote_forall2_In
-    .
-  End Instances.
+  #[export] Instance quote_For_all_usual {P s} {quote_elt : ground_quotable elt} {quote_P : forall x, ground_quotable (P x:Prop)} {qP : quotation_of P} {qs : quotation_of s} : ground_quotable (For_all P s)
+    := quote_For_all.
+  Definition quote_Exists_dec_usual {P} (P_dec : forall x, {P x} + {~P x}) {s} {quote_elt : ground_quotable elt} {qP_dec : quotation_of P_dec} {quote_P : forall x, ground_quotable (P x:Prop)} {qP : quotation_of P} {qs : quotation_of s} : ground_quotable (Exists P s)
+    := quote_Exists_dec P_dec.
+  #[export] Instance quote_forall2_In_usual {P s} {qP : quotation_of P} {qs : quotation_of s} {quote_elt : ground_quotable elt} {quote_P : forall x y, ground_quotable (P x y:Prop)} : ground_quotable (forall v1 v2, In v1 s -> In v2 s -> P v1 v2) := _.
 End QuoteUsualWSetsOn.
 
-Module QuoteUsualSetsOn (E : UsualOrderedType) (Import M : SetsOn E).
-  Module QM := QuoteUsualWSetsOn E M.
-  Module QM' := QuoteSetsOn E M.
+Module Type UsualSets <: Sets.
+  Declare Module E : UsualOrderedType.
+  Include SetsOn E.
+End UsualSets.
 
-  Module Definitions := QM.Definitions <+ QM'.OnlyOrdDefinitions.
-  Include Definitions.
-
-  Module Export Instances := QM.Instances <+ QM'.OnlyOrdInstances.
+Module QuoteUsualSetsOn (Import M : UsualSets) (MProperties : OrdPropertiesSig M) (qE : QuotationOfUsualOrderedType M.E) (qM : QuotationOfSets M) (qMProperties : QuotationOfOrdProperties M MProperties qE).
+  Include QuoteSets M MProperties qE qM qMProperties.
+  Module InnerQuoteUsualSetsOn := QuoteUsualWSetsOn M.E M MProperties.P qE qM qMProperties.qP.
+  Export (hints) InnerQuoteUsualSetsOn.
 End QuoteUsualSetsOn.
 
-Module QuoteSetsOnWithLeibniz (E : OrderedTypeWithLeibniz) (Import M : SetsOn E).
-  Module Import QM := QuoteSetsOn E M.
+Module Type QuotationOfOrderedTypeWithLeibniz (T : OrderedTypeWithLeibniz).
+  Include QuotationOfOrderedType T.
+  #[export] Declare Instance qeq_leibniz : quotation_of T.eq_leibniz.
+End QuotationOfOrderedTypeWithLeibniz.
 
-  Module Definitions.
-    Notation quote_In := QM.quote_In.
-    Notation quote_Equal := QM.quote_Equal.
-    Notation quote_Subset := QM.quote_Subset.
-    Notation quote_Empty := QM.quote_Empty.
-    Notation quote_Add := QM.quote_Add.
-    Notation quote_neg_In := QM.quote_neg_In.
-    Notation quote_neg_Equal := QM.quote_neg_Equal.
-    Notation quote_neg_Subset := QM.quote_neg_Subset.
-    Notation quote_neg_Empty := QM.quote_neg_Empty.
-    Notation quote_neg_Add := QM.quote_neg_Add.
-    Notation quote_Above := QM.quote_Above.
-    Notation quote_Below := QM.quote_Below.
+Module QuoteSWithLeibniz (Import M : SWithLeibniz) (MProperties : OrdPropertiesSig M) (qE : QuotationOfOrderedTypeWithLeibniz M.E) (qM : QuotationOfSets M) (qMProperties : QuotationOfOrdProperties M MProperties qE).
+  Include QuoteSets M MProperties qE qM qMProperties.
 
+  #[local] Instance all_P_Proper {P : E.t -> Prop} : Proper (E.eq ==> Basics.impl) P.
+  Proof.
+    intros ?? H.
+    apply E.eq_leibniz in H; subst; exact id.
+  Defined.
+  #[export] Instance qall_P_Proper : quotation_of (@all_P_Proper) := ltac:(unfold_quotation_of (); exact _).
 
-    #[local] Instance all_P_Proper {P : E.t -> Prop} : Proper (E.eq ==> Basics.impl) P.
-    Proof.
-      intros ?? H.
-      apply E.eq_leibniz in H; subst; exact id.
-    Defined.
+  #[export] Instance quote_For_all_leibniz {P s} {quote_elt : ground_quotable elt} {quote_P : forall x, ground_quotable (P x:Prop)} {qP : quotation_of P} {qs : quotation_of s} : ground_quotable (For_all P s)
+    := quote_For_all.
+  Definition quote_Exists_dec_leibniz {P} (P_dec : forall x, {P x} + {~P x}) {s} {quote_elt : ground_quotable elt} {qP_dec : quotation_of P_dec} {quote_P : forall x, ground_quotable (P x:Prop)} {qP : quotation_of P} {qs : quotation_of s} : ground_quotable (Exists P s)
+    := quote_Exists_dec P_dec.
+  #[export] Instance quote_forall2_In_leibniz {P s} {qP : quotation_of P} {qs : quotation_of s} {quote_elt : ground_quotable elt} {quote_P : forall x y, ground_quotable (P x y:Prop)} : ground_quotable (forall v1 v2, In v1 s -> In v2 s -> P v1 v2) := _.
+End QuoteSWithLeibniz.
 
-    Section with_quote.
-      Context {qelt : quotation_of elt} {qt : quotation_of t}
-              {qIn : quotation_of In}
-              {qeq_dec : quotation_of eq_dec}
-              {qsubset_spec : quotation_of subset_spec}
-              {qempty : quotation_of empty}
-              {qadd : quotation_of add} {qelements : quotation_of elements}.
+Module QuoteMSetList (T : OrderedType) (Import M : MSetList.MakeSig T) (Import MOrdProperties : OrdPropertiesSig M) (Import qT : QuotationOfOrderedType T) (Import qM : MSetList.QuotationOfMake T M) (qMOrdProperties : QuotationOfOrdProperties M MOrdProperties qT).
+  Export (hints) qT qM qMOrdProperties.
+  Include QuoteSets M MOrdProperties qT qM qMOrdProperties.
 
-      #[export] Instance quote_For_all {P s} {quote_elt : ground_quotable elt} {quote_P : forall x, ground_quotable (P x:Prop)} {qP : quotation_of P} {qs : quotation_of s} : ground_quotable (For_all P s)
-        := QM.quote_For_all.
-      Definition quote_Exists_dec {P} (P_dec : forall x, {P x} + {~P x}) {s} {quote_elt : ground_quotable elt} {qP_dec : quotation_of P_dec} {quote_P : forall x, ground_quotable (P x:Prop)} {qP : quotation_of P} {qs : quotation_of s} : ground_quotable (Exists P s)
-        := QM.quote_Exists_dec P_dec.
-      #[export] Instance quote_forall2_In {P s} {qP : quotation_of P} {qs : quotation_of s} {quote_elt : ground_quotable elt} {quote_P : forall x y, ground_quotable (P x y:Prop)} : ground_quotable (forall v1 v2, In v1 s -> In v2 s -> P v1 v2) := _.
-    End with_quote.
-  End Definitions.
-
-  Include Definitions.
-
-  Module Export Instances.
-    #[export] Existing Instances
-     QM.quote_In
-     QM.quote_Equal
-     QM.quote_Subset
-     QM.quote_Empty
-     QM.quote_Add
-     QM.quote_neg_In
-     QM.quote_neg_Equal
-     QM.quote_neg_Subset
-     QM.quote_neg_Empty
-     QM.quote_neg_Add
-     quote_For_all
-     quote_forall2_In
-     QM.quote_Above
-     QM.quote_Below
-    .
-  End Instances.
-End QuoteSetsOnWithLeibniz.
-
-Module Type MSetList_MakeSig (T : OrderedType). Include MSetList.Make T. End MSetList_MakeSig.
-
-Module QuoteMSetList (E : OrderedType) (Import M : MSetList_MakeSig E).
-  Module Import QM := QuoteSetsOn E M.
-
-  Module OnlyMSetListDefinitions.
-    #[export] Instance quote_Ok {qE_compare : quotation_of E.compare} {qE_t : quotation_of E.t} {v} : ground_quotable (Raw.Ok v) := ltac:(cbv [Raw.Ok]; exact _).
-
-    #[export] Instance quote_t_ {qE_t : quotation_of E.t} {qE_compare : quotation_of E.compare} {quoteE_t : ground_quotable E.t} {qM_Mkt : quotation_of M.Mkt} : ground_quotable t_ := ltac:(destruct 1; exact _).
-  End OnlyMSetListDefinitions.
-
-  Module Definitions := QM.Definitions <+ OnlyMSetListDefinitions.
-  Include Definitions.
-
-  Module OnlyMSetListInstances.
-    #[export] Existing Instances
-     quote_Ok
-     quote_t_
-    .
-  End OnlyMSetListInstances.
-
-  Module Export Instances := QM.Instances <+ OnlyMSetListInstances.
+  Module Raw.
+    #[export] Instance quote_Ok {v} : ground_quotable (M.Raw.Ok v) := ltac:(cbv [M.Raw.Ok]; exact _).
+  End Raw.
+  Export (hints) Raw.
+  #[export] Instance quote_t_ {quoteE_t : ground_quotable E.t} : ground_quotable t_ := ltac:(destruct 1; exact _).
 End QuoteMSetList.
 
-Module QuoteMSetListWithLeibniz (E : OrderedTypeWithLeibniz) (Import M : MSetList_MakeSig E).
-  Module QM := QuoteSetsOnWithLeibniz E M.
-  Module QM' := QuoteMSetList E M.
-
-  Module Definitions := QM.Definitions <+ QM'.OnlyMSetListDefinitions.
-  Include Definitions.
-
-  Module Export Instances := QM.Instances <+ QM'.OnlyMSetListInstances.
+Module QuoteMSetListWithLeibniz (T : OrderedTypeWithLeibniz) (Import M : MSetList.MakeWithLeibnizSig T) (Import MOrdProperties : OrdPropertiesSig M) (Import qT : QuotationOfOrderedTypeWithLeibniz T) (Import qM : MSetList.QuotationOfMakeWithLeibniz T M) (qMOrdProperties : QuotationOfOrdProperties M MOrdProperties qT).
+  Export (hints) qT qM qMOrdProperties.
+  Include QuoteMSetList T M MOrdProperties qT qM qMOrdProperties.
+  Module InnerQuoteMSetListWithLeibniz := QuoteSWithLeibniz M MOrdProperties qT qM qMOrdProperties.
+  Export (hints) InnerQuoteMSetListWithLeibniz.
 End QuoteMSetListWithLeibniz.
